DY/Bytes/AttackerKnowledge.lean
@@ -1,0 +1,109 @@
+import DY.Kleene
+import DY.Bytes.Type
+import DY.Bytes.EquationalTheory
+import DY.Trace.Type
+
+namespace DY
+
+def EquationalTheories.mapTheories [EquationalTheories] {α: Type u} (f: TheoryId → α): List α :=
+  EquationalTheories.theories.mapFinIdx (fun id _ h_id =>
+    f (Fin.mk id h_id)
+  )
+
+theorem EquationalTheories.mem_mapTheories
+  {α: Type u}
+  [EquationalTheories]
+  (f: TheoryId → α)
+  (x: α)
+  :
+  (x ∈ EquationalTheories.mapTheories f) ↔
+  (exists id, f id = x)
+  := by
+    simp [mapTheories]
+    constructor
+    · intro ⟨ id, h_id, h⟩
+      exists Fin.mk id h_id
+    · intro ⟨ id, h_id ⟩
+      exists id.val
+      exists id.isLt
+
+-- TODO: messages sent on network
+def Bytes.AttackerKnows.pred [EquationalTheories] (tr: Trace α): Kleene.Set Bytes → Kleene.Set Bytes :=
+  (Kleene.combine (EquationalTheories.mapTheories (fun id =>
+    Kleene.combine (EquationalTheories.theories[id].attackerKnowledge.map AttackerKnowledge.pred)
+  )))
+
+theorem Bytes.AttackerKnows.pred_is_scott_continuous
+  [EquationalTheories]
+  (tr: Trace α)
+  :
+  Kleene.IsScottContinuous (Bytes.AttackerKnows.pred tr)
+  := by
+    unfold pred
+    apply Kleene.combine_isScottContinuous
+    simp only [EquationalTheories.mem_mapTheories, forall_exists_index]
+    intros _ id h
+    subst h
+    apply Kleene.combine_isScottContinuous
+    simp only [List.mem_map, forall_exists_index, and_imp, forall_apply_eq_imp_iff₂]
+    intro attKnowledge h_attKnowledge
+    exact attKnowledge.pred_scott_continuous
+
+def Bytes.AttackerKnows [EquationalTheories] (b: Bytes) (tr: Trace α): Prop :=
+  Kleene.mkWeakestFixpoint (Bytes.AttackerKnows.pred tr) b
+
+theorem Bytes.AttackerKnows.prove
+  [EquationalTheories]
+  (theory: EquationalTheory)
+  [inst: HasEquationalTheory theory]
+  (att: AttackerKnowledge)
+  (b: Bytes) (tr: Trace α)
+  :
+    att ∈ theory.attackerKnowledge →
+    att.pred (Bytes.AttackerKnows · tr) b →
+    Bytes.AttackerKnows b tr
+  := by
+    apply theory.into_theory_id
+    generalize HasEquationalTheory.id theory = id
+    clear inst
+    unfold AttackerKnows
+    intro h_att h_b
+    rewrite [← Kleene.mkWeakestFixpoint_is_fixpoint (pred tr) (AttackerKnows.pred_is_scott_continuous tr)]
+    unfold pred
+    simp only [Kleene.combine]
+    exists Kleene.combine (EquationalTheories.theories[id].attackerKnowledge.map AttackerKnowledge.pred)
+    constructor
+    · simp only [EquationalTheories.mapTheories, List.mem_mapFinIdx]
+      exists id.val
+      exists id.isLt
+    simp only [Kleene.combine]
+    exists att.pred
+    grind
+
+theorem Bytes.AttackerKnows.is_least_fixpoint
+  [EquationalTheories]
+  (pred: Bytes → Prop)
+  (h_pred:
+    ∀ (id: TheoryId) att out,
+      att ∈ EquationalTheories.theories[id].attackerKnowledge →
+      att.pred pred out →
+      pred out
+  )
+  (b: Bytes) (tr: Trace α)
+  :
+    Bytes.AttackerKnows b tr →
+    pred b
+  :=
+    Kleene.mkWeakestFixpoint_is_weakest (AttackerKnows.pred tr) (AttackerKnows.pred_is_scott_continuous tr) pred (by
+      simp only [Subset, AttackerKnows.pred]
+      intro b
+      simp [Kleene.combine, EquationalTheories.mem_mapTheories]
+      grind
+    ) b
+
+theorem Bytes.AttackerKnows.pred_trace_erase [EquationalTheories] (tr: Trace α):
+  Bytes.AttackerKnows.pred tr = Bytes.AttackerKnows.pred (tr.erase)
+  := by
+    simp [Bytes.AttackerKnows.pred]
+
+end DY
