DY/Bytes/EquationalTheory.lean
@@ -1,0 +1,231 @@
+import DY.Bytes.Type
+import DY.Kleene
+
+namespace DY
+
+structure AttackerKnowledge [BytesCtors] where
+  pred: (Bytes → Prop) → Bytes → Prop
+  pred_scott_continuous: DY.Kleene.IsScottContinuous pred
+
+structure EquationalTheory where
+  ctors: List BytesCtor
+  attackerKnowledge:
+    [BytesCtors] → [Bytes.HasCtors ctors] →
+    List AttackerKnowledge
+
+-- This typeclass is useful in the following situation:
+-- def myEqThy: EquationalTheory where
+--   ctors := myCtors
+--   attackerKnowledge := ...
+-- Then there is a mismatch between
+--   Bytes.HasCtors myCtors
+-- (typeclass needed by functions before we define equational theories)
+-- and
+--   Bytes.HasCtors myEqThy.ctors
+-- (through the instance of HasEquationalTheory myEqThy)
+class EquationalTheory.CtorsEq (theory: semiOutParam EquationalTheory) (ctors: List BytesCtor) where
+  pf: theory.ctors = ctors
+
+instance: EquationalTheory.CtorsEq theory theory.ctors where
+  pf := rfl
+
+class EquationalTheories where
+  theories: List EquationalTheory
+
+abbrev TheoryId [EquationalTheories]: Type := Fin (EquationalTheories.theories.length)
+
+def BytesCtors.ofList (ctorsList: List BytesCtor): BytesCtors where
+  n := ctorsList.length
+  ctors i := ctorsList[i]
+
+instance [EquationalTheories]: BytesCtors := BytesCtors.ofList (EquationalTheories.theories.flatMap EquationalTheory.ctors)
+
+def computeCtorIndex (l: List EquationalTheory) (i: Nat): Nat :=
+  match l, i with
+  | [], _ => 0
+  | _, 0 => 0
+  | h::t, i+1 =>
+    h.ctors.length + computeCtorIndex t i
+
+theorem computeCtorIndex_in_bounds (l: List EquationalTheory) (i: Nat) (j: Nat) (h_i: i < l.length) (h_j: j < l[i].ctors.length):
+  computeCtorIndex l i + j < (l.flatMap EquationalTheory.ctors).length
+  := by
+    induction l generalizing i with
+    | nil => grind
+    | cons h t ih =>
+      cases i with
+      | zero =>
+        simp [computeCtorIndex]
+        grind
+      | succ i =>
+        have := ih i (by grind) (by grind)
+        simp [computeCtorIndex]
+        simp_all +arith
+
+theorem computeCtorIndex_getElem (l: List EquationalTheory) (i: Nat) (j: Nat) (h_i: i < l.length) (h_j: j < l[i].ctors.length):
+  (l.flatMap EquationalTheory.ctors)[computeCtorIndex l i + j]'(computeCtorIndex_in_bounds l i j h_i h_j) = l[i].ctors[j]
+  := by
+    induction l generalizing i with
+    | nil => grind
+    | cons h t ih =>
+      cases i with
+      | zero =>
+        simp [computeCtorIndex]
+        grind
+      | succ i =>
+        have := ih i (by grind) (by grind)
+        simp [computeCtorIndex]
+        grind
+
+
+class HasEquationalTheory [EquationalTheories] (theory: EquationalTheory) where
+  id: TheoryId
+  pf: EquationalTheories.theories[id] = theory
+
+instance [EquationalTheories] (id: TheoryId): HasEquationalTheory (EquationalTheories.theories[id]) where
+  id := id
+  pf := rfl
+
+theorem HasEquationalTheory.ext
+  [EquationalTheories]
+  (theory1 theory2: EquationalTheory)
+  [inst1: HasEquationalTheory theory1]
+  [inst2: HasEquationalTheory theory2]
+  :
+    inst1.id = inst2.id →
+    inst1 ≍ inst2
+  := by
+    cases inst1
+    cases inst2
+    grind
+
+def EquationalTheory.into_theory_id
+  [EquationalTheories]
+  (theory: EquationalTheory)
+  [inst: HasEquationalTheory theory]
+  (P: (theory: EquationalTheory) → [HasEquationalTheory theory] → Sort u)
+  (x: P EquationalTheories.theories[inst.id])
+  : P theory
+  := by
+    suffices h : P EquationalTheories.theories[inst.id] = P theory by
+      rewrite [← h]
+      exact x
+    have := inst.pf
+    congr
+    apply HasEquationalTheory.ext
+    simp [HasEquationalTheory.id]
+
+def EquationalTheory.toGlobalIndex [EquationalTheories] (theory: EquationalTheory) [HasEquationalTheory theory] (id: Fin theory.ctors.length): Fin BytesCtors.n :=
+  Fin.mk (computeCtorIndex EquationalTheories.theories (HasEquationalTheory.id theory) + (id.val)) (by
+      have := computeCtorIndex_in_bounds EquationalTheories.theories (HasEquationalTheory.id theory) (id.val) (by grind) (by
+        have := @HasEquationalTheory.pf _ theory _
+        simp_all
+      )
+      unfold BytesCtors.n instBytesCtorsOfEquationalTheories BytesCtors.ofList
+      assumption
+    )
+
+def EquationalTheory.toGlobalIndex_correct [EquationalTheories] (theory: EquationalTheory) [HasEquationalTheory theory] (id: Fin theory.ctors.length):
+  BytesCtors.ctors (theory.toGlobalIndex id) = theory.ctors[id]
+  := by
+    have := computeCtorIndex_getElem EquationalTheories.theories (HasEquationalTheory.id theory) (id.val) (by grind) (by
+      have := @HasEquationalTheory.pf _ theory _
+      simp_all
+    )
+    unfold BytesCtors.ctors instBytesCtorsOfEquationalTheories BytesCtors.ofList EquationalTheory.toGlobalIndex
+    have := @HasEquationalTheory.pf _ theory _
+    simp_all
+
+structure EquationalTheories.CtorId [EquationalTheories] where
+  idThy: TheoryId
+  idCtor: Fin (EquationalTheories.theories[idThy].ctors.length)
+
+def fromGlobalIndexAux (l: List EquationalTheory) (id: Nat): Nat × Nat :=
+  match l with
+  | [] => (0, 0) -- unreachable
+  | h::t =>
+    if id < h.ctors.length then (0, id)
+    else
+      let (x, y) := fromGlobalIndexAux t (id - h.ctors.length)
+      (x+1, y)
+
+def fromGlobalIndexAux_in_bounds_1 (l: List EquationalTheory) (id: Nat)
+  (h_id: id < (BytesCtors.ofList (l.flatMap EquationalTheory.ctors)).n)
+  :
+  (fromGlobalIndexAux l id).1 < l.length
+  := by
+    fun_induction fromGlobalIndexAux <;>
+    grind [BytesCtors.n, BytesCtors.ofList]
+
+def fromGlobalIndexAux_in_bounds_2 (l: List EquationalTheory) (id: Nat)
+  (h_id: id < (BytesCtors.ofList (l.flatMap EquationalTheory.ctors)).n)
+  :
+  (fromGlobalIndexAux l id).2 < (l[(fromGlobalIndexAux l id).1]'(fromGlobalIndexAux_in_bounds_1 l id h_id)).ctors.length
+  := by
+    fun_induction fromGlobalIndexAux <;>
+    grind [fromGlobalIndexAux, BytesCtors.n, BytesCtors.ofList]
+
+def fromGlobalIndex [EquationalTheories] (id: CtorId): EquationalTheories.CtorId where
+  idThy := Fin.mk (fromGlobalIndexAux EquationalTheories.theories id).1 (fromGlobalIndexAux_in_bounds_1 EquationalTheories.theories id.val id.isLt)
+  idCtor := Fin.mk (fromGlobalIndexAux EquationalTheories.theories id).2 (fromGlobalIndexAux_in_bounds_2 EquationalTheories.theories id.val id.isLt)
+
+theorem fromGlobalIndexAux_correct
+  (l: List EquationalTheory) (id: Nat)
+  (h_id: id < (BytesCtors.ofList (l.flatMap EquationalTheory.ctors)).n)
+  : (l[(fromGlobalIndexAux l id).1]'(fromGlobalIndexAux_in_bounds_1 l id h_id)).ctors[(fromGlobalIndexAux l id).2]'(fromGlobalIndexAux_in_bounds_2 l id h_id) = (BytesCtors.ofList (l.flatMap EquationalTheory.ctors)).ctors (Fin.mk id h_id)
+  := by
+    fun_induction fromGlobalIndexAux
+    · grind [fromGlobalIndexAux, BytesCtors.n, BytesCtors.ofList]
+    · simp_all [fromGlobalIndexAux, BytesCtors.n, BytesCtors.ofList]
+    · simp only [BytesCtors.ofList, List.flatMap_cons, BytesCtors.n] at h_id
+      simp_all [fromGlobalIndexAux, BytesCtors.n, BytesCtors.ofList]
+      grind
+
+theorem fromGlobalIndex_correct
+  [EquationalTheories]
+  (id: CtorId)
+  : EquationalTheories.theories[(fromGlobalIndex id).idThy].ctors[(fromGlobalIndex id).idCtor] = (BytesCtors.ctors id)
+  := by
+    apply fromGlobalIndexAux_correct EquationalTheories.theories id.val id.isLt
+
+theorem fromGlobalIndexAux_roundtrip
+  (l: List EquationalTheory)
+  (idThy: Nat) (idCtor: Nat)
+  (h_idThy: idThy < l.length)
+  (h_idCtor: idCtor < l[idThy].ctors.length)
+  : (fromGlobalIndexAux l ((computeCtorIndex l idThy) + idCtor)) = (idThy, idCtor)
+  := by
+    fun_induction computeCtorIndex
+    · unfold List.length at h_idThy
+      simp_all
+    · unfold fromGlobalIndexAux
+      grind
+    · simp_all [fromGlobalIndexAux]
+      grind
+
+theorem fromGlobalIndex_roundtrip
+  [EquationalTheories]
+  (idThy: TheoryId) (idCtor: Fin (EquationalTheories.theories[idThy].ctors.length))
+  : (fromGlobalIndex (EquationalTheories.theories[idThy].toGlobalIndex idCtor)) = {idThy, idCtor}
+  := by
+    unfold fromGlobalIndex EquationalTheory.toGlobalIndex
+    have := fromGlobalIndexAux_roundtrip EquationalTheories.theories idThy.val idCtor.val idThy.isLt idCtor.isLt
+    simp_all [HasEquationalTheory.id]
+    obtain ⟨ idCtor, h_idCtor ⟩ := idCtor
+    grind
+
+instance [EquationalTheories] (theory: EquationalTheory) [HasEquationalTheory theory] [theory.CtorsEq ctors]: Bytes.HasCtors ctors where
+  tc id_thy := {
+    id := theory.toGlobalIndex (EquationalTheory.CtorsEq.pf (theory := theory) (ctors := ctors) ▸ id_thy)
+    pf := EquationalTheory.CtorsEq.pf (theory := theory) (ctors := ctors) ▸ theory.toGlobalIndex_correct (EquationalTheory.CtorsEq.pf (theory := theory) (ctors := ctors) ▸ id_thy)
+  }
+
+instance
+  [EquationalTheories]
+  (theory: EquationalTheory) [HasEquationalTheory theory]
+  (id: Fin theory.ctors.length)
+  : Bytes.HasCtorAt (theory.toGlobalIndex id) theory.ctors[id]
+  where
+    pf := theory.toGlobalIndex_correct id
+
+end DY
