DY/Bytes/EquationalTheoryInvariants.lean
@@ -1,0 +1,63 @@
+import DY.Bytes.Invariants
+import DY.Bytes.EquationalTheory
+import DY.Bytes.AttackerKnowledge
+
+namespace DY
+
+def AttackerKnowledge.PreservesPublishability [BytesCtors] [BytesCtorsInvariants] (attKnows: AttackerKnowledge) :=
+  ∀ out tr,
+    attKnows.pred (Bytes.Publishable · tr) out →
+    Bytes.Publishable out tr
+
+structure EquationalTheory.PreservesPublishability [EquationalTheories] [BytesCtorsInvariants] (theory: EquationalTheory) [HasEquationalTheory theory] where
+  pf: ∀ attKnows, attKnows ∈ theory.attackerKnowledge → attKnows.PreservesPublishability
+
+structure EquationalTheoryInvariants [EquationalTheories] (theory: EquationalTheory) where
+  invariant: (id: Fin theory.ctors.length) → BytesCtorInvariants.Internal theory.ctors[id]
+
+class EquationalTheoryInvariants.Has [EquationalTheories] [BytesCtorsInvariants] {theory: EquationalTheory} [HasEquationalTheory theory] (eqInvs: EquationalTheoryInvariants theory) where
+  pf: ∀ id, eqInvs.invariant id = (theory.toGlobalIndex_correct id) ▸ (BytesCtorsInvariants.funs (theory.toGlobalIndex id))
+
+class EquationalTheories.Invariants [EquationalTheories] where
+  invariants: (id: TheoryId) → EquationalTheoryInvariants EquationalTheories.theories[id]
+
+instance [EquationalTheories] [EquationalTheories.Invariants]: BytesCtorsInvariants where
+  funs id :=
+    let idEqThy := fromGlobalIndex id
+    let res: BytesCtorInvariants.Internal (BytesCtors.ctors id) := (fromGlobalIndex_correct id ▸ (EquationalTheories.Invariants.invariants idEqThy.idThy).invariant idEqThy.idCtor)
+    res
+
+instance [EquationalTheories] [EquationalTheories.Invariants] (idThy: TheoryId): (EquationalTheories.Invariants.invariants idThy).Has where
+  pf idCtor := by
+    unfold BytesCtorsInvariants.funs instBytesCtorsInvariantsOfInvariants
+    have := fromGlobalIndex_roundtrip idThy
+    grind
+
+def EquationalTheoryInvariants.mkHasBytesInvariants
+  [EquationalTheories] [EquationalTheories.Invariants]
+  {theory: EquationalTheory} [HasEquationalTheory theory]
+  (invariants: EquationalTheoryInvariants theory)
+  [inst: invariants.Has]
+  (id: Fin theory.ctors.length)
+  : HasBytesInvariants (theory.toGlobalIndex id) (invariants.invariant id)
+  where
+    pf := by
+      simp [BytesCtorsInvariants.funs, inst.pf id]
+      simp [BytesCtorInvariants.into]
+      sorry
+
+class EquationalTheories.PreservesPublishability [EquationalTheories] [EquationalTheories.Invariants] where
+  pf: (id: TheoryId) → EquationalTheories.theories[id].PreservesPublishability
+
+theorem attacker_only_knows_publishable_values
+  [EquationalTheories] [EquationalTheories.Invariants] [EquationalTheories.PreservesPublishability]
+  (b: Bytes) (tr: ProofTrace)
+  :
+    b.AttackerKnows tr →
+    b.Publishable tr
+  := by
+    apply Bytes.AttackerKnows.is_least_fixpoint (Bytes.Publishable · tr)
+    intro id att out h_att h_out
+    exact (EquationalTheories.PreservesPublishability.pf id).pf att h_att out tr h_out
+
+end DY
