DY/Bytes/Invariants.lean
@@ -1,0 +1,315 @@
+import DY.Bytes.Type
+import DY.Label
+import DY.Trace
+
+namespace DY
+-- Well formed
+
+def BytesWellFormedT [BytesCtors] := ProofTrace → Prop
+def BytesWellFormedT.default [BytesCtors]: BytesWellFormedT := fun _ => False
+
+class BytesWellFormed [BytesCtors] where
+  funs: BytesFunCtors BytesWellFormedT
+
+def Bytes.wellFormed [BytesCtors] [BytesWellFormed] (b: Bytes) : BytesWellFormedT :=
+  Bytes.mkRec BytesWellFormed.funs .default b
+
+class HasBytesWellFormed [BytesCtors] [BytesWellFormed] (id: CtorId) {ctor: BytesCtor} [Bytes.HasCtorAt id ctor] (binv: outParam (BytesFunCtor id BytesWellFormedT)) where
+  pf: BytesWellFormed.funs id = binv.into
+  dummy: Unit -- leanprover/lean4#11477 workaround
+
+theorem Bytes.wellFormed.eq
+  [BytesCtors] [tc_binv: BytesWellFormed]
+  (id: CtorId) {ctor: BytesCtor} [Bytes.HasCtorAt id ctor]
+  {binv: BytesFunCtor id BytesWellFormedT}
+  [tc: HasBytesWellFormed id binv]
+  (b: BytesView id)
+  (tr: ProofTrace)
+  : Bytes.wellFormed (b.pack) tr = binv.func b.data b.dataBytes Bytes.wellFormed tr
+  := by
+    have lem {a b} (f g: a → b) (x: a): f = g → f x = g x := by grind
+    apply lem
+    apply Bytes.mkRec.eqView
+    exact tc.pf
+
+grind_pattern Bytes.wellFormed.eq => Bytes.wellFormed (b.pack) tr
+
+-- Usage
+
+structure Usage [BytesCtors] where
+  type: String
+  tag: String
+  data: Option Bytes
+
+def Usage.nothing [BytesCtors]: Usage where
+  type := ""
+  tag := ""
+  data := none
+
+def GetUsageT [BytesCtors] := ProofTrace → Usage
+def GetUsageT.default [BytesCtors]: GetUsageT := fun _ => Usage.nothing
+
+class GetUsage [BytesCtors] where
+  funs: BytesFunCtors GetUsageT
+
+noncomputable
+def Bytes.usage [BytesCtors] [GetUsage] (b: Bytes) : GetUsageT :=
+  Bytes.mkRec GetUsage.funs .default b
+
+class HasGetUsage [BytesCtors] [GetUsage] (id: CtorId) {ctor: BytesCtor} [Bytes.HasCtorAt id ctor] (binv: outParam (BytesFunCtor id GetUsageT)) where
+  pf: GetUsage.funs id = binv.into
+  dummy: Unit -- leanprover/lean4#11477 workaround
+
+theorem Bytes.usage.eq
+  [BytesCtors] [tc_binv: GetUsage]
+  (id: CtorId) {ctor: BytesCtor} [Bytes.HasCtorAt id ctor]
+  {binv: BytesFunCtor id GetUsageT}
+  [tc: HasGetUsage id binv]
+  (b: BytesView id)
+  (tr: ProofTrace)
+  : Bytes.usage (b.pack) tr = binv.func b.data b.dataBytes Bytes.usage tr
+  := by
+    have lem {a b} (f g: a → b) (x: a): f = g → f x = g x := by grind
+    apply lem
+    apply Bytes.mkRec.eqView
+    exact tc.pf
+
+grind_pattern Bytes.usage.eq => Bytes.usage (b.pack) tr
+
+-- Usage later
+
+def GetUsageLaterT [BytesCtors] (x: BytesWellFormedT × GetUsageT) :=
+  let (wf, usg) := x
+  ∀ tr1 tr2: ProofTrace, tr1 ≤ tr2 → wf tr1 → usg tr1 = usg tr2
+
+class GetUsageLater [BytesCtors] [BytesWellFormed] [GetUsage] where
+  proofs: BytesFunCtorsProof2 BytesWellFormed.funs GetUsage.funs GetUsageLaterT
+
+theorem Bytes.usage_later
+  [BytesCtors] [BytesWellFormed] [GetUsage] [GetUsageLater]
+  (b: Bytes)
+  (tr1 tr2: ProofTrace)
+  :
+  tr1 ≤ tr2 →
+  Bytes.wellFormed b tr1 →
+  Bytes.usage b tr1 = Bytes.usage b tr2
+  := by
+    apply GetUsageLater.proofs.prove
+
+grind_pattern Bytes.usage_later => Bytes.usage b tr1, tr1 ≤ tr2
+
+-- Label
+
+def GetLabelT [BytesCtors] := ProofTrace → Label
+def GetLabelT.default [BytesCtors]: GetLabelT := fun _ => Label.secret
+
+class GetLabel [BytesCtors] where
+  funs: BytesFunCtors GetLabelT
+
+noncomputable
+def Bytes.label [BytesCtors] [GetLabel] (b: Bytes) : GetLabelT :=
+  Bytes.mkRec GetLabel.funs .default b
+
+class HasGetLabel [BytesCtors] [GetLabel] (id: CtorId) {ctor: BytesCtor} [Bytes.HasCtorAt id ctor] (binv: outParam (BytesFunCtor id GetLabelT)) where
+  pf: GetLabel.funs id = binv.into
+  dummy: Unit -- leanprover/lean4#11477 workaround
+
+theorem Bytes.label.eq
+  [BytesCtors] [tc_binv: GetLabel]
+  (id: CtorId) {ctor: BytesCtor} [Bytes.HasCtorAt id ctor]
+  {binv: BytesFunCtor id GetLabelT}
+  [tc: HasGetLabel id binv]
+  (b: BytesView id)
+  (tr: ProofTrace)
+  : Bytes.label (b.pack) tr = binv.func b.data b.dataBytes Bytes.label tr
+  := by
+    have lem {a b} (f g: a → b) (x: a): f = g → f x = g x := by grind
+    apply lem
+    apply Bytes.mkRec.eqView
+    exact tc.pf
+
+grind_pattern Bytes.label.eq => Bytes.label (b.pack) tr
+
+-- Label later
+
+def GetLabelLaterT [BytesCtors] (x: BytesWellFormedT × GetLabelT) :=
+  let (wf, usg) := x
+  ∀ tr1 tr2: ProofTrace, tr1 ≤ tr2 → wf tr1 → usg tr1 = usg tr2
+
+class GetLabelLater [BytesCtors] [BytesWellFormed] [GetLabel] where
+  proofs: BytesFunCtorsProof2 BytesWellFormed.funs GetLabel.funs GetLabelLaterT
+
+theorem Bytes.label_later
+  [BytesCtors] [BytesWellFormed] [GetLabel] [GetLabelLater]
+  (b: Bytes)
+  (tr1 tr2: ProofTrace)
+  :
+  tr1 ≤ tr2 →
+  Bytes.wellFormed b tr1 →
+  Bytes.label b tr1 = Bytes.label b tr2
+  := by
+    apply GetLabelLater.proofs.prove
+
+grind_pattern Bytes.label_later => Bytes.label b tr1, tr1 ≤ tr2
+
+-- Invariant
+
+def BytesInvariantT [BytesCtors] := ProofTrace → Prop
+
+def BytesInvariantT.default [BytesCtors]: BytesInvariantT := fun _ => False
+
+class BytesInvariant [BytesCtors] where
+  funs: BytesFunCtors BytesInvariantT
+
+def Bytes.invariant [BytesCtors] [BytesInvariant] (b: Bytes) (tr: ProofTrace) : Prop :=
+  Bytes.mkRec BytesInvariant.funs .default b tr
+
+class HasBytesInvariant [BytesCtors] [BytesInvariant] (id: CtorId) {ctor: BytesCtor} [Bytes.HasCtorAt id ctor] (binv: outParam (BytesFunCtor id BytesInvariantT)) where
+  pf: BytesInvariant.funs id = binv.into
+  dummy: Unit -- leanprover/lean4#11477 workaround
+
+theorem Bytes.invariant.eq
+  [BytesCtors] [tc_binv: BytesInvariant]
+  (id: CtorId) {ctor: BytesCtor} [Bytes.HasCtorAt id ctor]
+  {binv: BytesFunCtor id BytesInvariantT}
+  [tc: HasBytesInvariant id binv]
+  (b: BytesView id)
+  (tr: ProofTrace)
+  : Bytes.invariant (b.pack) tr = binv.func b.data b.dataBytes Bytes.invariant tr
+  := by
+    have lem {a b} (f g: a → b) (x: a): f = g → f x = g x := by grind
+    apply lem
+    apply Bytes.mkRec.eqView
+    exact tc.pf
+
+grind_pattern Bytes.invariant.eq => Bytes.invariant (b.pack) tr
+
+-- Invariant implies well formed
+
+def BytesInvariantImpliesBytesWellFormedT [BytesCtors] (x: BytesInvariantT × BytesWellFormedT) :=
+  let (binv, bwf) := x
+  ∀ tr, binv tr → bwf tr
+
+class BytesInvariantImpliesBytesWellFormed [BytesCtors] [BytesWellFormed] [BytesInvariant] where
+  proofs: BytesFunCtorsProof2 BytesInvariant.funs BytesWellFormed.funs BytesInvariantImpliesBytesWellFormedT
+
+theorem Bytes.invariant_implies_wellformed
+  [BytesCtors] [BytesWellFormed] [BytesInvariant] [BytesInvariantImpliesBytesWellFormed]
+  (b: Bytes)
+  (tr: ProofTrace)
+  :
+  Bytes.invariant b tr →
+  Bytes.wellFormed b tr
+  := by
+    apply BytesInvariantImpliesBytesWellFormed.proofs.prove
+
+grind_pattern Bytes.invariant_implies_wellformed => Bytes.wellFormed b tr, Bytes.invariant b tr
+
+-- Invariant later
+
+def BytesInvariantLaterT [BytesCtors] (binv: BytesInvariantT) :=
+  ∀ tr1 tr2, tr1 ≤ tr2 → binv tr1 → binv tr2
+
+class BytesInvariantLater [BytesCtors] [BytesInvariant] where
+  proofs: BytesFunCtorsProof1 BytesInvariant.funs BytesInvariantLaterT
+
+theorem Bytes.invariant.later
+  [BytesCtors] [BytesInvariant] [BytesInvariantLater]
+  (b: Bytes)
+  (tr1 tr2: ProofTrace)
+  :
+  tr1 ≤ tr2 →
+  Bytes.invariant b tr1 →
+  Bytes.invariant b tr2
+  := by
+    apply BytesInvariantLater.proofs.prove
+
+grind_pattern Bytes.invariant.later => Bytes.invariant b tr1, tr1 ≤ tr2
+
+structure BytesCtorInvariants.Internal [BytesCtors] (ctor: BytesCtor) where
+  well_formed: BytesFunCtor.Internal ctor BytesWellFormedT
+
+  usage: BytesFunCtor.Internal ctor GetUsageT
+  usage_later: BytesFunCtorProof2.Internal well_formed usage GetUsageLaterT
+
+  label: [GetUsage] → BytesFunCtor.Internal ctor GetLabelT
+  label_later: [BytesWellFormed] → [GetUsage] → [GetUsageLater] → BytesFunCtorProof2.Internal well_formed label GetLabelLaterT
+
+  invariant: [GetUsage] → [GetLabel] → BytesFunCtor.Internal ctor BytesInvariantT
+  invariant_implies_wellformed: [GetUsage] → [GetLabel] → BytesFunCtorProof2.Internal invariant well_formed BytesInvariantImpliesBytesWellFormedT
+  invariant_later: [GetUsage] → [GetLabel] → BytesFunCtorProof1.Internal invariant BytesInvariantLaterT
+  -- ...
+
+def BytesCtorInvariants.ById [BytesCtors] (id: CtorId) := BytesCtorInvariants.Internal (BytesCtors.ctors id)
+def BytesCtorInvariants [BytesCtors] (id: CtorId) {ctor: BytesCtor} [Bytes.HasCtorAt id ctor] := BytesCtorInvariants.Internal ctor
+
+def BytesCtorInvariants.into
+  [BytesCtors] {id: CtorId} {ctor: BytesCtor} [Bytes.HasCtorAt id ctor]
+  (f: BytesCtorInvariants id)
+  : BytesCtorInvariants.ById id
+  where
+    well_formed := BytesFunCtor.into f.well_formed
+
+    usage := BytesFunCtor.into f.usage
+    usage_later := BytesFunCtorProof2.into f.usage_later
+
+    label := BytesFunCtor.into f.label
+    label_later := BytesFunCtorProof2.into f.label_later
+
+    invariant := BytesFunCtor.into f.invariant
+    invariant_implies_wellformed := BytesFunCtorProof2.into f.invariant_implies_wellformed
+    invariant_later := BytesFunCtorProof1.into f.invariant_later
+
+
+class BytesCtorsInvariants [BytesCtors] where
+  funs: (id: CtorId) → BytesCtorInvariants.ById id
+
+instance [BytesCtors] [BytesCtorsInvariants]: BytesWellFormed where
+  funs id := (BytesCtorsInvariants.funs id).well_formed
+
+instance [BytesCtors] [BytesCtorsInvariants]: GetUsage where
+  funs id := (BytesCtorsInvariants.funs id).usage
+
+instance [BytesCtors] [BytesCtorsInvariants]: GetUsageLater where
+  proofs id := (BytesCtorsInvariants.funs id).usage_later
+
+instance [BytesCtors] [BytesCtorsInvariants]: GetLabel where
+  funs id := (BytesCtorsInvariants.funs id).label
+
+instance [BytesCtors] [BytesCtorsInvariants]: GetLabelLater where
+  proofs id := (BytesCtorsInvariants.funs id).label_later
+
+instance [BytesCtors] [BytesCtorsInvariants]: BytesInvariant where
+  funs id := (BytesCtorsInvariants.funs id).invariant
+
+instance [BytesCtors] [BytesCtorsInvariants]: BytesInvariantImpliesBytesWellFormed where
+  proofs id := (BytesCtorsInvariants.funs id).invariant_implies_wellformed
+
+instance [BytesCtors] [BytesCtorsInvariants]: BytesInvariantLater where
+  proofs id := (BytesCtorsInvariants.funs id).invariant_later
+
+class HasBytesInvariants [BytesCtors] [BytesCtorsInvariants] (id: CtorId) {ctor: BytesCtor} [Bytes.HasCtorAt id ctor] (funs: outParam (BytesCtorInvariants id)) where
+  pf: BytesCtorsInvariants.funs id = funs.into
+
+instance [BytesCtors] [BytesCtorsInvariants] (id: CtorId) {ctor: BytesCtor} [Bytes.HasCtorAt id ctor] (funs: BytesCtorInvariants id) [tc: HasBytesInvariants id funs]: HasBytesWellFormed id funs.well_formed where
+  pf := by simp only [BytesWellFormed.funs, tc.pf, BytesCtorInvariants.into]
+  dummy := ()
+
+instance [BytesCtors] [BytesCtorsInvariants] (id: CtorId) {ctor: BytesCtor} [Bytes.HasCtorAt id ctor] (funs: BytesCtorInvariants id) [tc: HasBytesInvariants id funs]: HasGetUsage id funs.usage where
+  pf := by simp only [GetUsage.funs, tc.pf, BytesCtorInvariants.into]
+  dummy := ()
+
+instance [BytesCtors] [BytesCtorsInvariants] (id: CtorId) {ctor: BytesCtor} [Bytes.HasCtorAt id ctor] (funs: BytesCtorInvariants id) [tc: HasBytesInvariants id funs]: HasGetLabel id funs.label where
+  pf := by simp only [GetLabel.funs, tc.pf, BytesCtorInvariants.into]
+  dummy := ()
+
+instance [BytesCtors] [BytesCtorsInvariants] (id: CtorId) {ctor: BytesCtor} [Bytes.HasCtorAt id ctor] (funs: BytesCtorInvariants id) [tc: HasBytesInvariants id funs]: HasBytesInvariant id funs.invariant where
+  pf := by simp only [BytesInvariant.funs, tc.pf, BytesCtorInvariants.into]
+  dummy := ()
+
+@[grind]
+def Bytes.Publishable [BytesCtors] [BytesCtorsInvariants] (b: Bytes) (tr: ProofTrace) :=
+  b.invariant tr ∧
+  (b.label tr).canFlow Label.pub tr
+
+end DY
