DY/Bytes/Type.lean
@@ -1,0 +1,518 @@
+namespace DY
+
+structure BytesCtor where
+  data: Type 0
+  nBytes: Nat
+  -- TODO: we might want to move these outside BytesCtor(s) so that they only contain typing information
+  dataOrd: Ord data
+  dataReflOrd: Std.ReflOrd data
+  dataLawfulEqOrd: Std.LawfulEqOrd data
+  dataOrientedOrd: Std.OrientedOrd data
+  dataTransOrd: Std.TransOrd data
+
+-- TODO: if we want to compute bytes term, this Vect type is slow for performance
+-- because it contains the length of each subvector (classic issue)
+-- we cannot use list + subtype because Lean tries to unfold it into a big mutually recursive type
+-- (see https://lean-lang.org/doc/reference/latest/find/?domain=Verso.Genre.Manual.section&name=nested-inductive-types )
+-- possible solution: Use List or Vector (no length constraints),
+-- but then subtype Bytes by the fact that each length is correct?
+inductive Vect (a:Type u): Nat -> Type u where
+  | nil: Vect a 0
+  | cons: a -> Vect a n -> Vect a (n+1)
+
+syntax "V[" withoutPosition(term,*,?) "]"  : term
+
+macro_rules
+  | `(V[ $elems,* ]) => do
+    pure (← elems.getElems.foldrM (fun elem acc => ``(Vect.cons $elem $acc)) (← ``(Vect.nil)))
+
+class BytesCtors where
+  n: Nat
+  ctors: Fin n -> BytesCtor
+
+abbrev CtorId [BytesCtors] := Fin BytesCtors.n
+
+structure Bytes [BytesCtors] where
+  id: CtorId
+  data: (BytesCtors.ctors id).data
+  dataBytes: Vect (Bytes) ((BytesCtors.ctors id).nBytes)
+
+mutual
+def compareVectBytes [BytesCtors] {n: Nat} (v1 v2: Vect Bytes n): Ordering :=
+  match v1, v2 with
+  | .nil, .nil => .eq
+  | .cons h1 t1, .cons h2 t2 =>
+    match compareBytes h1 h2 with
+    | .lt => .lt
+    | .gt => .gt
+    | .eq => compareVectBytes t1 t2
+def compareBytes [BytesCtors] (b1 b2: Bytes): Ordering :=
+  let {id := id1, data := data1, dataBytes := dataBytes1} := b1
+  let {id := id2, data := data2, dataBytes := dataBytes2} := b2
+  match h: compare id1 id2 with
+  | .lt => .lt
+  | .gt => .gt
+  | .eq => by
+    simp at h
+    subst h
+    generalize BytesCtors.ctors id1 = ctor at *
+    exact (
+      match ctor.dataOrd.compare data1 data2 with
+      | .lt => .lt
+      | .gt => .gt
+      | .eq => (
+        compareVectBytes dataBytes1 dataBytes2
+      )
+    )
+end
+
+instance [BytesCtors] {id: CtorId}: Ord ((BytesCtors.ctors id).data) := (BytesCtors.ctors id).dataOrd
+instance [BytesCtors] {id: CtorId}: Std.ReflOrd ((BytesCtors.ctors id).data) := (BytesCtors.ctors id).dataReflOrd
+instance [BytesCtors] {id: CtorId}: Std.LawfulEqOrd ((BytesCtors.ctors id).data) := (BytesCtors.ctors id).dataLawfulEqOrd
+instance [BytesCtors] {id: CtorId}: Std.OrientedOrd ((BytesCtors.ctors id).data) := (BytesCtors.ctors id).dataOrientedOrd
+instance [BytesCtors] {id: CtorId}: Std.TransOrd ((BytesCtors.ctors id).data) := (BytesCtors.ctors id).dataTransOrd
+
+mutual
+theorem compareVectBytes_Refl
+  [BytesCtors] {n: Nat}
+  (v: Vect Bytes n)
+  : compareVectBytes v v = .eq
+  := by
+    cases v
+    · rfl
+    · rename_i h t
+      unfold compareVectBytes
+      simp [compareBytes_Refl h, compareVectBytes_Refl t]
+
+theorem compareBytes_Refl
+  [BytesCtors]
+  (b: Bytes)
+  : compareBytes b b = .eq
+  := by
+    let {id := id, data := data, dataBytes := dataBytes} := b
+    simp only [compareBytes]
+    have id_Refl : compare id id = .eq := by simp
+    rewrite [id_Refl]
+    dsimp only
+    simp [compareVectBytes_Refl]
+end
+
+mutual
+theorem compareVectBytes_LawfulEq
+  [BytesCtors] {n: Nat}
+  (v1 v2: Vect Bytes n)
+  : compareVectBytes v1 v2 = .eq → v1 = v2
+  := by
+    cases v1 <;> cases v2
+    · simp [compareVectBytes]
+    · simp [compareVectBytes]
+      split
+      · simp
+      · simp
+      · rename_i heq
+        have := compareBytes_LawfulEq _ _ heq
+        intro heq
+        have := compareVectBytes_LawfulEq _ _ heq
+        simp_all
+
+theorem compareBytes_LawfulEq
+  [BytesCtors]
+  (b1 b2: Bytes)
+  : compareBytes b1 b2 = .eq → b1 = b2
+  := by
+    let {id := id1, data := data1, dataBytes := dataBytes1} := b1
+    let {id := id2, data := data2, dataBytes := dataBytes2} := b2
+    simp only [compareBytes, Bytes.mk.injEq]
+    split
+    · simp
+    · simp
+    rename_i heq
+    have heq := Std.LawfulEqOrd.eq_of_compare heq
+    subst heq
+    dsimp only
+    split
+    · simp
+    · simp
+    rename_i heq
+    have := Std.LawfulEqOrd.eq_of_compare heq
+    intro heq
+    have := compareVectBytes_LawfulEq _ _ heq
+    grind
+end
+
+mutual
+theorem compareVectBytes_Oriented
+  [BytesCtors] {n: Nat}
+  (v1 v2: Vect Bytes n)
+  : compareVectBytes v1 v2 = (compareVectBytes v2 v1).swap
+  := by
+    cases v1 <;> cases v2
+    · simp [compareVectBytes]
+    · rename_i h1 t1 h2 t2
+      simp only [compareVectBytes]
+      have := compareBytes_Oriented h1 h2
+      split
+      · split <;> simp_all
+      · split <;> simp_all
+      have := compareVectBytes_Oriented t1 t2
+      split <;> simp_all
+
+theorem compareBytes_Oriented
+  [BytesCtors]
+  (b1 b2: Bytes)
+  : compareBytes b1 b2 = (compareBytes b2 b1).swap
+  := by
+    let {id := id1, data := data1, dataBytes := dataBytes1} := b1
+    let {id := id2, data := data2, dataBytes := dataBytes2} := b2
+    simp only [compareBytes]
+    have id_swap: compare id1 id2 = (compare id2 id1).swap := Std.OrientedOrd.eq_swap
+    split
+    · split <;> grind
+    · split <;> grind
+    rename_i heq
+    have heq' := Std.LawfulEqOrd.eq_of_compare heq
+    subst heq'
+    dsimp only
+    have data_swap: compare data1 data2 = (compare data2 data1).swap := Std.OrientedOrd.eq_swap
+    split
+    · split <;> grind
+    · split <;> grind
+    have dataBytes_swap := compareVectBytes_Oriented dataBytes1 dataBytes2
+    split <;> grind
+end
+
+theorem mkTransitive
+  {a: Type u}
+  (r: a → a → Ordering)
+  (hlawful: ∀ x y, (r x y) = .eq → x = y)
+  (htranslt: ∀ x y z, (r x y) = .lt → (r y z) = .lt → (r x z) = .lt)
+  : ∀ x y z, (r x y).isLE → (r y z).isLE → (r x z).isLE
+  := by
+    intros x y z
+    simp only [Ordering.isLE]
+    grind [cases Ordering]
+
+mutual
+theorem compareVectBytes_TransLt
+  [BytesCtors] {n: Nat}
+  (v1 v2 v3: Vect Bytes n)
+  : (compareVectBytes v1 v2) = .lt → (compareVectBytes v2 v3) = .lt → (compareVectBytes v1 v3) = .lt
+  := by
+    cases v1 <;> cases v2 <;> cases v3
+    · simp [compareVectBytes]
+    · rename_i h1 t1 h2 t2 h3 t3
+      simp only [compareVectBytes]
+      intros h12 h23
+      split at h12 <;> rename_i h_cmp12
+      · split at h23 <;> rename_i h_cmp23
+        · have := compareBytes_TransLt h1 h2 h3 h_cmp12 h_cmp23
+          grind
+        · contradiction
+        · have h_eq23 := compareBytes_LawfulEq h2 h3 h_cmp23
+          grind
+      · contradiction
+      · have h_eq12 := compareBytes_LawfulEq h1 h2 h_cmp12
+        subst h_eq12
+        split at h23 <;> rename_i h_cmp23
+        · rfl
+        · contradiction
+        · exact compareVectBytes_TransLt t1 t2 t3 h12 h23
+
+theorem compareBytes_TransLt
+  [BytesCtors]
+  (b1 b2 b3: Bytes)
+  : (compareBytes b1 b2) = .lt → (compareBytes b2 b3) = .lt → (compareBytes b1 b3) = .lt
+  := by
+    let {id := id1, data := data1, dataBytes := dataBytes1} := b1
+    let {id := id2, data := data2, dataBytes := dataBytes2} := b2
+    let {id := id3, data := data3, dataBytes := dataBytes3} := b3
+    simp only [compareBytes]
+    intro h12 h23
+    split at h12 <;> rename_i h_id12
+    · split at h23 <;> rename_i h_id23
+      · have := Std.TransCmp.lt_trans h_id12 h_id23
+        grind
+      · contradiction
+      · grind
+    · contradiction
+    · split at h23 <;> rename_i h_id23
+      · grind
+      · contradiction
+      · have h_id12_eq := Std.LawfulEqOrd.eq_of_compare h_id12
+        have h_id23_eq := Std.LawfulEqOrd.eq_of_compare h_id23
+        subst h_id12_eq
+        subst h_id23_eq
+        dsimp only at *
+        rewrite [h_id12]
+        dsimp only
+        split at h12 <;> rename_i h_data12
+        · split at h23 <;> rename_i h_data23
+          · have := Std.TransCmp.lt_trans h_data12 h_data23
+            grind
+          · contradiction
+          · grind
+        · contradiction
+        · split at h23 <;> rename_i h_data23
+          · grind
+          · contradiction
+          · have h_data12_eq := Std.LawfulEqOrd.eq_of_compare h_data12
+            have h_data23_eq := Std.LawfulEqOrd.eq_of_compare h_data23
+            subst h_data12_eq
+            subst h_data23_eq
+            simp [compareVectBytes_TransLt dataBytes1 dataBytes2 dataBytes3 h12 h23]
+end
+
+theorem compareBytes_Trans
+  [BytesCtors]
+  (b1 b2 b3: Bytes)
+  : (compareBytes b1 b2).isLE → (compareBytes b2 b3).isLE → (compareBytes b1 b3).isLE
+  := mkTransitive compareBytes compareBytes_LawfulEq compareBytes_TransLt b1 b2 b3
+
+instance [BytesCtors]: Ord Bytes where
+  compare := compareBytes
+
+instance [BytesCtors]: Std.ReflOrd Bytes where
+  compare_self {b} := compareBytes_Refl b
+
+instance [BytesCtors]: Std.LawfulEqOrd Bytes where
+  eq_of_compare {a b} := compareBytes_LawfulEq a b
+
+instance [BytesCtors]: Std.OrientedOrd Bytes where
+  eq_swap {a b} := compareBytes_Oriented a b
+
+instance [BytesCtors]: Std.TransOrd Bytes where
+  isLE_trans {a b c} := compareBytes_Trans a b c
+
+instance [BytesCtors]: DecidableEq Bytes :=
+  fun b1 b2 =>
+    if h: compare b1 b2 = .eq then
+      .isTrue (Std.LawfulEqOrd.eq_of_compare h)
+    else
+      .isFalse (by
+        intro h_eq
+        subst h_eq
+        exact (h Std.ReflOrd.compare_self)
+      )
+
+instance [BytesCtors]: LE Bytes := leOfOrd
+
+class Bytes.HasCtorAt [BytesCtors] (id: CtorId) (ctor: outParam BytesCtor) where
+  pf: BytesCtors.ctors id = ctor
+
+class Bytes.HasCtor [BytesCtors] (ctor: BytesCtor) where
+  id: CtorId
+  pf: BytesCtors.ctors id = ctor
+
+instance [BytesCtors] {ctor} [tc: Bytes.HasCtor ctor]: Bytes.HasCtorAt tc.id ctor where
+  pf := tc.pf
+
+class Bytes.HasCtors [BytesCtors] (ctors: List BytesCtor) where
+  tc: (id: Fin ctors.length) → Bytes.HasCtor ctors[id]
+
+structure BytesView [BytesCtors] (id: CtorId) {ctor: BytesCtor} [Bytes.HasCtorAt id ctor] where
+  data: ctor.data
+  dataBytes: Vect Bytes ctor.nBytes
+
+def Bytes.view? [BytesCtors] (b: Bytes) (id: CtorId) {ctor: BytesCtor} [tc: Bytes.HasCtorAt id ctor] : Option (BytesView id) :=
+  if h_id: b.id = id then
+    some {
+      data := tc.pf ▸ h_id ▸ b.data
+      dataBytes := tc.pf ▸ h_id ▸ b.dataBytes,
+    }
+  else
+    none
+
+def BytesView.pack
+  [BytesCtors]
+  (id: CtorId) {ctor: BytesCtor} [tc: Bytes.HasCtorAt id ctor]
+  (b: BytesView id)
+  : Bytes
+  :=
+  {
+    id := id,
+    data := tc.pf ▸ b.data,
+    dataBytes := tc.pf ▸ b.dataBytes,
+  }
+
+theorem Bytes.pack_view?
+  [BytesCtors]
+  (b: Bytes)
+  (id: CtorId) {ctor: BytesCtor} [tc: Bytes.HasCtorAt id ctor]
+  :
+  match b.view? id with
+  | some bview => bview.pack = b
+  | none => True
+  := by
+    simp only [BytesView.pack, Bytes.view?]
+    cases b
+    grind
+
+grind_pattern Bytes.pack_view? => b.view? id
+
+theorem BytesView.view_pack
+  [BytesCtors] {id: CtorId} {ctor: BytesCtor} [Bytes.HasCtorAt id ctor]
+  (b: BytesView id)
+  : (b.pack).view? id = some b
+  := by
+    simp only [BytesView.pack, Bytes.view?]
+    cases b
+    grind
+
+grind_pattern BytesView.view_pack => b.pack
+
+structure BytesFunCtor.Internal [BytesCtors] (ctor: BytesCtor) (a: Type u) where
+  func: ctor.data → Vect Bytes ctor.nBytes → (Bytes → a) → a
+  func_wf:
+    ∀ data dataBytes rec1 rec2,
+      (∀ b, sizeOf b < sizeOf dataBytes → rec1 b = rec2 b) →
+      func data dataBytes rec1 = func data dataBytes rec2
+
+def BytesFunCtor.ById [BytesCtors] (id: CtorId) (a: Type u) := BytesFunCtor.Internal (BytesCtors.ctors id) a
+def BytesFunCtor [BytesCtors] (id: CtorId) {ctor: BytesCtor} [Bytes.HasCtorAt id ctor] (a: Type u) := BytesFunCtor.Internal ctor a
+
+def BytesFunCtor.into
+  [BytesCtors] {id: CtorId} {a: Type u} {ctor: BytesCtor} [Bytes.HasCtorAt id ctor]
+  (f: BytesFunCtor id a)
+  : BytesFunCtor.ById id a
+  :=
+  {
+    func data dataBytes rec := f.func (@Bytes.HasCtorAt.pf _ id _ _ ▸ data) (@Bytes.HasCtorAt.pf _ id _ _ ▸ dataBytes) rec
+    func_wf := @Bytes.HasCtorAt.pf _ id ctor _ ▸ f.func_wf
+  }
+
+def BytesFunCtors [BytesCtors] (a: Type u) :=
+  (id: CtorId) → BytesFunCtor.ById id a
+
+noncomputable
+def Bytes.mkRec
+  [BytesCtors]
+  {a: Type u}
+  (funs: BytesFunCtors a)
+  (default: a)
+  (b: Bytes)
+  : a
+  :=
+    let {id, data, dataBytes} := b
+    (funs id).func data dataBytes (fun bChild =>
+      if sizeOf bChild < sizeOf dataBytes then
+        mkRec funs default bChild
+      else
+        default
+    )
+
+theorem Bytes.mkRec.eq
+  [BytesCtors]
+  {a: Type u}
+  (funs: BytesFunCtors a)
+  (default: a)
+  (b: Bytes)
+  : Bytes.mkRec funs default b = (funs b.id).func b.data b.dataBytes (Bytes.mkRec funs default)
+  := by
+    unfold Bytes.mkRec
+    cases b
+    rename_i id data dataBytes
+    apply (funs id).func_wf
+    grind
+
+theorem Bytes.mkRec.eqView
+  [BytesCtors]
+  (id: CtorId) {ctor: BytesCtor} [Bytes.HasCtorAt id ctor]
+  {a: Type u}
+  (funs: BytesFunCtors a)
+  (default: a)
+  (func: BytesFunCtor id a)
+  (pf: funs id = func.into)
+  (b: BytesView id)
+  : Bytes.mkRec funs default (b.pack) = func.func b.data b.dataBytes (Bytes.mkRec funs default)
+  := by
+    rewrite [Bytes.mkRec.eq funs default b.pack]
+    simp_all [BytesView.pack, BytesFunCtor.into]
+    grind
+
+def Bytes.Proof [BytesCtors] (p: Bytes → Prop) :=
+  ∀ id data dataBytes,
+    (∀ b, sizeOf b < sizeOf dataBytes → p b) →
+    p ({id, data, dataBytes})
+
+theorem Bytes.proveRec
+  [BytesCtors]
+  (p: Bytes → Prop)
+  (pf: Bytes.Proof p)
+  (b: Bytes)
+  : p b
+  :=
+    let {id, data, dataBytes} := b
+    pf id data dataBytes (fun b _ => Bytes.proveRec p pf b)
+
+def BytesFunCtorProof1.Internal [BytesCtors] {ctor: BytesCtor} {a: Type u} (f: BytesFunCtor.Internal ctor a) (p: a → Prop) :=
+  ∀ data dataBytes rec,
+    (∀ b, sizeOf b < sizeOf dataBytes → p (rec b)) →
+    p (f.func data dataBytes rec)
+
+def BytesFunCtorProof1.ById [BytesCtors] {id: CtorId} {a: Type u} (f: BytesFunCtor.ById id a) (p: a → Prop) := BytesFunCtorProof1.Internal f p
+
+def BytesFunCtorProof1 [BytesCtors] {id: CtorId} {ctor: BytesCtor} [Bytes.HasCtorAt id ctor] {a: Type u} (f: BytesFunCtor id a) (p: a → Prop) := BytesFunCtorProof1.Internal f p
+
+def BytesFunCtorProof1.into
+  [BytesCtors] {id: CtorId} {ctor: BytesCtor} [Bytes.HasCtorAt id ctor] {a: Type u}
+  {f: BytesFunCtor id a} {p: a → Prop}
+  (pf: BytesFunCtorProof1 f p)
+  : BytesFunCtorProof1.ById f.into p
+  := fun data dataBytes rec pfRec =>
+    pf (@Bytes.HasCtorAt.pf _ id _ _ ▸ data) (@Bytes.HasCtorAt.pf _ id _ _ ▸ dataBytes) rec (@Bytes.HasCtorAt.pf _ id _ _ ▸ pfRec)
+
+def BytesFunCtorsProof1 [BytesCtors] {a: Type u} (f: BytesFunCtors a) (p: a → Prop) :=
+  (id: CtorId) → BytesFunCtorProof1.ById (f id) p
+
+def BytesFunCtorsProof1.prove
+  [BytesCtors]
+  {a: Type u}
+  {funs: BytesFunCtors a}
+  {p: a → Prop}
+  (pfuns: BytesFunCtorsProof1 funs p)
+  (default: a)
+  (b: Bytes)
+  : p (Bytes.mkRec funs default b)
+  := by
+    apply Bytes.proveRec (fun b => p (Bytes.mkRec funs default b))
+    intros id data dataBytes pfRec
+    rewrite [Bytes.mkRec.eq funs default {id, data, dataBytes}]
+    exact pfuns _ _ _ _ pfRec
+
+def BytesFunCtorProof2.Internal [BytesCtors] {ctor: BytesCtor} {a: Type u} {b: Type v} (f1: BytesFunCtor.Internal ctor a) (f2: BytesFunCtor.Internal ctor b) (p: a × b → Prop) :=
+  ∀ data dataBytes rec1 rec2,
+    (∀ b, sizeOf b < sizeOf dataBytes → p (rec1 b, rec2 b)) →
+    p (f1.func data dataBytes rec1, f2.func data dataBytes rec2)
+
+def BytesFunCtorProof2.ById [BytesCtors] {id: CtorId} {a: Type u} {b: Type v} (f1: BytesFunCtor.ById id a) (f2: BytesFunCtor.ById id b) (p: a × b → Prop) := BytesFunCtorProof2.Internal f1 f2 p
+
+def BytesFunCtorProof2 [BytesCtors] {id: CtorId} {ctor: BytesCtor} [Bytes.HasCtorAt id ctor] {a: Type u} {b: Type v} (f1: BytesFunCtor id a) (f2: BytesFunCtor id b) (p: a × b → Prop) := BytesFunCtorProof2.Internal f1 f2 p
+
+def BytesFunCtorProof2.into
+  [BytesCtors] {id: CtorId} {ctor: BytesCtor} [Bytes.HasCtorAt id ctor] {a: Type u} {b: Type v}
+  {f1: BytesFunCtor id a} {f2: BytesFunCtor id b} {p: a × b → Prop}
+  (pf: BytesFunCtorProof2 f1 f2 p)
+  : BytesFunCtorProof2.ById f1.into f2.into p
+  := fun data dataBytes rec1 rec2 pfRec =>
+    pf (@Bytes.HasCtorAt.pf _ id _ _ ▸ data) (@Bytes.HasCtorAt.pf _ id _ _ ▸ dataBytes) rec1 rec2 (@Bytes.HasCtorAt.pf _ id _ _ ▸ pfRec)
+
+def BytesFunCtorsProof2 [BytesCtors] {a: Type u} {b: Type v} (f1: BytesFunCtors a) (f2: BytesFunCtors b) (p: a × b → Prop) :=
+  (id: CtorId) → BytesFunCtorProof2.ById (f1 id) (f2 id) p
+
+def BytesFunCtorsProof2.prove
+  [BytesCtors]
+  {a: Type u} {b: Type v}
+  {funs1: BytesFunCtors a} {funs2: BytesFunCtors b}
+  {p: a × b → Prop}
+  (pfuns: BytesFunCtorsProof2 funs1 funs2 p)
+  (default1: a)
+  (default2: b)
+  (b: Bytes)
+  : p (Bytes.mkRec funs1 default1 b, Bytes.mkRec funs2 default2 b)
+  := by
+    apply Bytes.proveRec (fun b => p (Bytes.mkRec funs1 default1 b, Bytes.mkRec funs2 default2 b))
+    intros id data dataBytes pfRec
+    rewrite [Bytes.mkRec.eq funs1 default1 {id, data, dataBytes}, Bytes.mkRec.eq funs2 default2 {id, data, dataBytes}]
+    exact pfuns _ _ _ _ _ pfRec
+
+end DY
