DY/EquationalTheory/Concat.lean
@@ -1,0 +1,356 @@
+import DY.Bytes.Type
+import DY.Label.Type
+import DY.Trace.Type
+import DY.Bytes.EquationalTheoryInvariants
+import DY.Bytes.AttackerKnowledge
+
+namespace DY
+
+class CanConcat (Bytes: Type u) where
+  concat: Bytes → Bytes → Bytes
+  -- TODO: index
+  split: Bytes → Option (Bytes × Bytes)
+
+export CanConcat (concat)
+export CanConcat (split)
+
+instance: Ord Unit where
+  compare _ _ := .eq
+
+instance: Std.ReflOrd Unit where
+  compare_self := by grind
+
+instance: Std.LawfulEqOrd Unit where
+  eq_of_compare := by grind
+
+instance: Std.OrientedOrd Unit where
+  eq_swap := by grind [Ordering.swap]
+
+instance: Std.TransOrd Unit where
+  isLE_trans := by grind
+
+-- Constructors
+
+abbrev Concat.ctor: BytesCtor where
+  data := Unit
+  nBytes := 2
+  dataOrd := inferInstance
+  dataReflOrd := inferInstance
+  dataLawfulEqOrd := inferInstance
+  dataOrientedOrd := inferInstance
+  dataTransOrd := inferInstance
+
+class abbrev Concat.HasCtor [BytesCtors] := Bytes.HasCtor Concat.ctor
+
+abbrev Concat.id [BytesCtors] [Concat.HasCtor]: CtorId := Bytes.HasCtor.id Concat.ctor
+
+abbrev Concat.View [BytesCtors] [Concat.HasCtor] := BytesView Concat.id
+
+instance [BytesCtors] [Concat.HasCtor]: CanConcat Bytes where
+  concat lhs rhs :=
+    ({
+      data := (),
+      dataBytes := V[lhs, rhs]
+    } : Concat.View).pack
+
+  split buf :=
+    match buf.view? Concat.id with
+    | some { data := (), dataBytes := V[lhs, rhs] } =>
+      some (lhs, rhs)
+    | none => none
+
+theorem split_concat
+  [BytesCtors] [Concat.HasCtor]
+  (lhs rhs: Bytes)
+  : split (concat lhs rhs) = some (lhs, rhs)
+  := by
+    simp only [split, concat]
+    grind
+
+theorem concat_split
+  [BytesCtors] [Concat.HasCtor]
+  (buf lhs rhs: Bytes)
+  : split buf = some (lhs, rhs) → concat lhs rhs = buf
+  := by
+    simp only [concat, split]
+    grind
+
+def Concat.ctors := [Concat.ctor]
+
+instance [BytesCtors] [tc: Bytes.HasCtors Concat.ctors]: Bytes.HasCtor Concat.ctor := tc.tc (Fin.mk 0 (by simp [Concat.ctors]))
+
+-- Equational theory
+
+def Concat.attKnowsConcat [BytesCtors] [Bytes.HasCtors Concat.ctors]: AttackerKnowledge where
+  pred p out :=
+    ∃ lhs rhs,
+      out = concat lhs rhs ∧
+      p lhs ∧
+      p rhs
+  pred_scott_continuous := by
+    sorry
+
+def Concat.attKnowsSplitLeft [BytesCtors] [Bytes.HasCtors Concat.ctors]: AttackerKnowledge where
+  pred p out :=
+    ∃ inp rhs,
+      some (out, rhs) = split inp ∧
+      p inp
+  pred_scott_continuous := by
+    sorry
+
+def Concat.attKnowsSplitRight [BytesCtors] [Bytes.HasCtors Concat.ctors]: AttackerKnowledge where
+  pred p out :=
+    ∃ inp lhs,
+      some (lhs, out) = split inp ∧
+      p inp
+  pred_scott_continuous := by
+    sorry
+
+def Concat.equationalTheory: EquationalTheory where
+  ctors := Concat.ctors
+  attackerKnowledge := [Concat.attKnowsConcat, Concat.attKnowsSplitLeft, Concat.attKnowsSplitRight]
+
+instance: EquationalTheory.CtorsEq Concat.equationalTheory Concat.ctors where pf := rfl
+
+instance: NeZero Concat.equationalTheory.ctors.length where
+  out := by simp [Concat.equationalTheory, Concat.ctors]
+
+theorem Concat.attacker_knows_concat
+  [EquationalTheories]
+  [HasEquationalTheory Concat.equationalTheory]
+  (lhs rhs: Bytes) (tr: Trace α)
+  :
+    lhs.AttackerKnows tr →
+    rhs.AttackerKnows tr →
+    (concat lhs rhs).AttackerKnows tr
+  := by
+    intro h_lhs h_rhs
+    apply Bytes.AttackerKnows.prove Concat.equationalTheory Concat.attKnowsConcat
+    · simp [Concat.equationalTheory]
+    simp only [Concat.attKnowsConcat]
+    grind
+
+theorem Concat.attacker_knows_split
+  [EquationalTheories]
+  [HasEquationalTheory Concat.equationalTheory]
+  (buf: Bytes) (tr: Trace α)
+  :
+    buf.AttackerKnows tr →
+    match split buf with
+    | none => True
+    | some (lhs, rhs) =>
+      lhs.AttackerKnows tr ∧
+      rhs.AttackerKnows tr
+  := by
+    intro h_buf
+    split
+    · trivial
+    rename_i lhs rhs _
+    constructor
+    · apply Bytes.AttackerKnows.prove Concat.equationalTheory Concat.attKnowsSplitLeft
+      · simp [Concat.equationalTheory]
+      simp only [Concat.attKnowsSplitLeft]
+      grind
+    · apply Bytes.AttackerKnows.prove Concat.equationalTheory Concat.attKnowsSplitRight
+      · simp [Concat.equationalTheory]
+      simp only [Concat.attKnowsSplitRight]
+      grind
+
+-- Invariants
+
+def Concat.invariants [BytesCtors]: BytesCtorInvariants.Internal Concat.ctor where
+  well_formed := {
+    func := fun () V[lhs, rhs] rec tr =>
+      rec lhs tr ∧ rec rhs tr
+    func_wf := by
+      intro data dataBytes rec1 rec2
+      let V[lhs, rhs] := dataBytes
+      simp_all +arith
+  }
+
+  usage := {
+    func data dataBytes rec tr := Usage.nothing
+    func_wf := by grind
+  }
+  usage_later data dataBytes rec_wf rec_usg := by grind [GetUsageLaterT]
+
+  label := {
+    func := fun () V[lhs, rhs] rec tr =>
+      Label.meet (rec lhs tr) (rec rhs tr)
+    func_wf := by
+      intro data dataBytes rec1 rec2
+      let V[lhs, rhs] := dataBytes
+      simp_all +arith
+  }
+  label_later data dataBytes rec_wf rec_usg := by
+    let V[lhs, rhs] := dataBytes
+    simp_all +arith [GetLabelLaterT]
+    grind
+
+  invariant := {
+    func := fun () V[lhs, rhs] rec tr =>
+      rec lhs tr ∧ rec rhs tr
+    func_wf := by
+      intro data dataBytes rec1 rec2
+      let V[lhs, rhs] := dataBytes
+      simp_all +arith
+  }
+  invariant_implies_wellformed data dataBytes rec_inv rec_wf := by
+    let V[lhs, rhs] := dataBytes
+    simp_all +arith [BytesInvariantImpliesBytesWellFormedT]
+  invariant_later data dataBytes rec := by
+    let V[lhs, rhs] := dataBytes
+    simp_all +arith [BytesInvariantLaterT]
+    grind
+
+theorem Concat.invariants.workaround_11309.invariant
+  [BytesCtors] [GetUsage] [GetLabel] [Concat.HasCtor]
+  : ∀ lhs rhs rec tr,
+    Concat.invariants.invariant.func () V[lhs, rhs] rec tr = (rec lhs tr ∧ rec rhs tr)
+  := by
+    intros
+    rfl
+
+class abbrev Concat.HasInvariants [BytesCtors] [Concat.HasCtor] [BytesCtorsInvariants] := HasBytesInvariants (Concat.id) Concat.invariants
+
+@[simp]
+theorem concat.wellFormed
+  [BytesCtors] [BytesCtorsInvariants]
+  [Concat.HasCtor] [Concat.HasInvariants]
+  (lhs rhs: Bytes) (tr: ProofTrace)
+  :
+    (concat lhs rhs).wellFormed tr = (lhs.wellFormed tr ∧ rhs.wellFormed tr)
+  := by
+    simp [concat, Bytes.wellFormed.eq, Concat.invariants]
+
+@[simp]
+theorem concat.label
+  [BytesCtors] [BytesCtorsInvariants]
+  [Concat.HasCtor] [Concat.HasInvariants]
+  (lhs rhs: Bytes) (tr: ProofTrace)
+  : (concat lhs rhs).label tr = Label.meet (lhs.label tr) (rhs.label tr)
+  := by
+    simp [concat, Bytes.label.eq, Concat.invariants]
+
+@[simp]
+theorem concat.invariant
+  [BytesCtors] [BytesCtorsInvariants]
+  [Concat.HasCtor] [Concat.HasInvariants]
+  (lhs rhs: Bytes) (tr: ProofTrace)
+  : (concat lhs rhs).invariant tr = (lhs.invariant tr ∧ rhs.invariant tr)
+  := by
+    simp [concat, Bytes.invariant.eq, Concat.invariants]
+
+
+@[simp]
+theorem split.wellFormed
+  [BytesCtors] [BytesCtorsInvariants]
+  [Concat.HasCtor] [Concat.HasInvariants]
+  (buf: Bytes) (tr: ProofTrace)
+  :
+    match split buf with
+    | none => True
+    | some (lhs, rhs) =>
+      buf.wellFormed tr = (lhs.wellFormed tr ∧ rhs.wellFormed tr)
+  := by
+    split
+    · trivial
+    rename_i lhs rhs heq
+    rewrite [← concat_split buf lhs rhs heq]
+    simp
+
+@[simp]
+theorem split.label
+  [BytesCtors] [BytesCtorsInvariants]
+  [Concat.HasCtor] [Concat.HasInvariants]
+  (buf: Bytes) (tr: ProofTrace)
+  :
+    match split buf with
+    | none => True
+    | some (lhs, rhs) =>
+      buf.label tr = Label.meet (lhs.label tr) (rhs.label tr)
+  := by
+    split
+    · trivial
+    rename_i lhs rhs heq
+    rewrite [← concat_split buf lhs rhs heq]
+    simp
+
+@[simp]
+theorem split.invariant
+  [BytesCtors] [BytesCtorsInvariants]
+  [Concat.HasCtor] [Concat.HasInvariants]
+  (buf: Bytes) (tr: ProofTrace)
+  :
+    buf.invariant tr →
+    match split buf with
+    | none => True
+    | some (lhs, rhs) =>
+      lhs.invariant tr ∧ rhs.invariant tr
+  := by
+    intro h_buf
+    split
+    · trivial
+    rename_i lhs rhs heq
+    rewrite [← concat_split buf lhs rhs heq] at h_buf
+    simp_all
+
+def Concat.EquationalTheoryInvariant [EquationalTheories]: EquationalTheoryInvariants Concat.equationalTheory where
+  invariant
+    | 0 => Concat.invariants
+
+instance
+  [EquationalTheories] [EquationalTheories.Invariants]
+  [HasEquationalTheory Concat.equationalTheory] [Concat.EquationalTheoryInvariant.Has]
+  : HasBytesInvariants Concat.id Concat.invariants :=
+  Concat.EquationalTheoryInvariant.mkHasBytesInvariants (Fin.mk 0 (by simp [Concat.equationalTheory, Concat.ctors]))
+
+-- Preserve publishability
+
+def Concat.attKnowsConcat.preserves_publishability
+  [BytesCtors] [BytesCtorsInvariants]
+  [Bytes.HasCtors Concat.ctors] [Concat.HasInvariants]: Concat.attKnowsConcat.PreservesPublishability :=
+  by
+    simp only [AttackerKnowledge.PreservesPublishability, Concat.attKnowsConcat]
+    intro out tr ⟨lhs, rhs, ⟨ h_out, h_lhs, h_rhs ⟩⟩
+    subst h_out
+    simp [Bytes.Publishable]
+    grind
+
+def Concat.attKnowsSplitLeft.preserves_publishability
+  [BytesCtors] [BytesCtorsInvariants]
+  [Bytes.HasCtors Concat.ctors] [Concat.HasInvariants]: Concat.attKnowsSplitLeft.PreservesPublishability :=
+  by
+    simp only [AttackerKnowledge.PreservesPublishability, Concat.attKnowsSplitLeft]
+    intro out tr ⟨inp, rhs, ⟨ h_out, h_inp ⟩⟩
+    simp_all [Bytes.Publishable]
+    have := split.label inp tr
+    have := split.invariant inp tr
+    grind
+
+def Concat.attKnowsSplitRight.preserves_publishability
+  [BytesCtors] [BytesCtorsInvariants]
+  [Bytes.HasCtors Concat.ctors] [Concat.HasInvariants]: Concat.attKnowsSplitRight.PreservesPublishability :=
+  by
+    simp only [AttackerKnowledge.PreservesPublishability, Concat.attKnowsSplitRight]
+    intro out tr ⟨inp, lhs, ⟨ h_out, h_inp ⟩⟩
+    simp_all [Bytes.Publishable]
+    have := split.label inp tr
+    have := split.invariant inp tr
+    grind
+
+def Concat.PreservesPublishability
+  [EquationalTheories] [EquationalTheories.Invariants]
+  [HasEquationalTheory Concat.equationalTheory]
+  [Concat.EquationalTheoryInvariant.Has]
+  : EquationalTheory.PreservesPublishability Concat.equationalTheory where
+  pf := by
+    unfold Concat.equationalTheory
+    simp
+    constructor
+    · exact attKnowsConcat.preserves_publishability
+    constructor
+    · exact attKnowsSplitLeft.preserves_publishability
+    · exact attKnowsSplitRight.preserves_publishability
+
+end DY
