DY/EquationalTheory/Hash.lean
@@ -1,0 +1,210 @@
+import DY.Bytes.Type
+import DY.Label.Type
+import DY.Trace.Type
+import DY.Bytes.EquationalTheoryInvariants
+import DY.Bytes.AttackerKnowledge
+
+namespace DY
+
+class CanHash (Bytes: Type u) where
+  hash: Bytes → Bytes
+
+export CanHash (hash)
+
+instance: Ord Unit where
+  compare _ _ := .eq
+
+instance: Std.ReflOrd Unit where
+  compare_self := by grind
+
+instance: Std.LawfulEqOrd Unit where
+  eq_of_compare := by grind
+
+instance: Std.OrientedOrd Unit where
+  eq_swap := by grind [Ordering.swap]
+
+instance: Std.TransOrd Unit where
+  isLE_trans := by grind
+
+-- Constructors
+
+abbrev Hash.ctor: BytesCtor where
+  data := Unit
+  nBytes := 1
+  dataOrd := inferInstance
+  dataReflOrd := inferInstance
+  dataLawfulEqOrd := inferInstance
+  dataOrientedOrd := inferInstance
+  dataTransOrd := inferInstance
+
+class abbrev Hash.HasCtor [BytesCtors] := Bytes.HasCtor Hash.ctor
+
+abbrev Hash.id [BytesCtors] [Hash.HasCtor]: CtorId := Bytes.HasCtor.id Hash.ctor
+
+abbrev Hash.View [BytesCtors] [Hash.HasCtor] := BytesView Hash.id
+
+instance [BytesCtors] [Hash.HasCtor]: CanHash Bytes where
+  hash inp :=
+    ({
+      data := (),
+      dataBytes := V[inp]
+    } : Hash.View).pack
+
+theorem hash_inj
+  [BytesCtors] [Hash.HasCtor]
+  (inp1 inp2: Bytes)
+  :
+    hash inp1 = hash inp2 →
+    inp1 = inp2
+  := by
+    simp only [hash]
+    grind
+
+def Hash.ctors := [Hash.ctor]
+
+instance [BytesCtors] [tc: Bytes.HasCtors Hash.ctors]: Bytes.HasCtor Hash.ctor := tc.tc (Fin.mk 0 (by simp [Hash.ctors]))
+
+-- Equational theory
+
+def Hash.attKnowsHash [BytesCtors] [Bytes.HasCtors Hash.ctors]: AttackerKnowledge where
+  pred p out :=
+    ∃ inp,
+      out = hash inp ∧
+      p inp
+  pred_scott_continuous := by
+    sorry
+
+def Hash.equationalTheory: EquationalTheory where
+  ctors := Hash.ctors
+  attackerKnowledge := [Hash.attKnowsHash]
+
+instance: EquationalTheory.CtorsEq Hash.equationalTheory Hash.ctors where pf := rfl
+
+instance: NeZero Hash.equationalTheory.ctors.length where
+  out := by simp [Hash.equationalTheory, Hash.ctors]
+
+theorem Hash.attacker_knows_hash
+  [EquationalTheories]
+  [HasEquationalTheory Hash.equationalTheory]
+  (inp: Bytes) (tr: Trace α)
+  :
+    inp.AttackerKnows tr →
+    (hash inp).AttackerKnows tr
+  := by
+    intro h_inp
+    apply Bytes.AttackerKnows.prove Hash.equationalTheory Hash.attKnowsHash
+    · simp [Hash.equationalTheory]
+    simp only [Hash.attKnowsHash]
+    grind
+
+-- Invariants
+
+def Hash.invariants [BytesCtors]: BytesCtorInvariants.Internal Hash.ctor where
+  well_formed := {
+    func := fun () V[inp] rec tr =>
+      rec inp tr
+    func_wf := by
+      intro data dataBytes rec1 rec2
+      let V[inp] := dataBytes
+      simp_all +arith
+  }
+
+  usage := {
+    func data dataBytes rec tr := Usage.nothing
+    func_wf := by grind
+  }
+  usage_later data dataBytes rec_wf rec_usg := by grind [GetUsageLaterT]
+
+  label := {
+    func := fun () V[inp] rec tr =>
+      rec inp tr
+    func_wf := by
+      intro data dataBytes rec1 rec2
+      let V[inp] := dataBytes
+      simp_all +arith
+  }
+  label_later data dataBytes rec_wf rec_usg := by
+    let V[inp] := dataBytes
+    simp_all +arith [GetLabelLaterT]
+    grind
+
+  invariant := {
+    func := fun () V[inp] rec tr =>
+      rec inp tr
+    func_wf := by
+      intro data dataBytes rec1 rec2
+      let V[inp] := dataBytes
+      simp_all +arith
+  }
+  invariant_implies_wellformed data dataBytes rec_inv rec_wf := by
+    let V[inp] := dataBytes
+    simp_all +arith [BytesInvariantImpliesBytesWellFormedT]
+  invariant_later data dataBytes rec := by
+    let V[inp] := dataBytes
+    simp_all +arith [BytesInvariantLaterT]
+    grind
+
+class abbrev Hash.HasInvariants [BytesCtors] [Hash.HasCtor] [BytesCtorsInvariants] := HasBytesInvariants (Hash.id) Hash.invariants
+
+@[simp]
+theorem hash.wellFormed
+  [BytesCtors] [BytesCtorsInvariants]
+  [Hash.HasCtor] [Hash.HasInvariants]
+  (inp: Bytes) (tr: ProofTrace)
+  :
+    (hash inp).wellFormed tr = inp.wellFormed tr
+  := by
+    simp [hash, Bytes.wellFormed.eq, Hash.invariants]
+
+@[simp]
+theorem hash.label
+  [BytesCtors] [BytesCtorsInvariants]
+  [Hash.HasCtor] [Hash.HasInvariants]
+  (inp: Bytes) (tr: ProofTrace)
+  : (hash inp).label tr = inp.label tr
+  := by
+    simp [hash, Bytes.label.eq, Hash.invariants]
+
+@[simp]
+theorem hash.invariant
+  [BytesCtors] [BytesCtorsInvariants]
+  [Hash.HasCtor] [Hash.HasInvariants]
+  (inp: Bytes) (tr: ProofTrace)
+  :
+    (hash inp).invariant tr =
+    inp.invariant tr
+  := by
+    simp [hash, Bytes.invariant.eq, Hash.invariants]
+
+def Hash.EquationalTheoryInvariant [EquationalTheories]: EquationalTheoryInvariants Hash.equationalTheory where
+  invariant
+    | 0 => Hash.invariants
+
+instance
+  [EquationalTheories] [EquationalTheories.Invariants]
+  [HasEquationalTheory Hash.equationalTheory] [Hash.EquationalTheoryInvariant.Has]
+  : HasBytesInvariants Hash.id Hash.invariants :=
+  Hash.EquationalTheoryInvariant.mkHasBytesInvariants (Fin.mk 0 (by simp [Hash.equationalTheory, Hash.ctors]))
+
+-- Preserve publishability
+
+def Hash.attKnowsHash.preserves_publishability
+  [BytesCtors] [BytesCtorsInvariants]
+  [Bytes.HasCtors Hash.ctors] [Hash.HasInvariants]: Hash.attKnowsHash.PreservesPublishability :=
+  by
+    simp only [AttackerKnowledge.PreservesPublishability, Hash.attKnowsHash]
+    intro out tr ⟨inp, ⟨ h_out, h_inp ⟩⟩
+    subst h_out
+    simp_all [Bytes.Publishable]
+
+def Hash.PreservesPublishability
+  [EquationalTheories] [EquationalTheories.Invariants]
+  [HasEquationalTheory Hash.equationalTheory]
+  [Hash.EquationalTheoryInvariant.Has]
+  : EquationalTheory.PreservesPublishability Hash.equationalTheory where
+  pf := by
+    unfold Hash.equationalTheory
+    simp
+    exact attKnowsHash.preserves_publishability
+
+end DY
