DY/EquationalTheory/Sign.lean
@@ -1,0 +1,362 @@
+import DY.Bytes.Type
+import DY.Label.Type
+import DY.Trace.Type
+import DY.Bytes.EquationalTheoryInvariants
+import DY.Bytes.AttackerKnowledge
+
+namespace DY
+
+class CanSign (Bytes: Type u) where
+  vk: Bytes → Bytes
+  -- sk nonce msg
+  sign: Bytes → Bytes → Bytes → Bytes
+  -- vk msg sig
+  verify: Bytes → Bytes → Bytes → Bool
+
+export CanSign (vk)
+export CanSign (sign)
+export CanSign (verify)
+
+instance: Ord Unit where
+  compare _ _ := .eq
+
+instance: Std.ReflOrd Unit where
+  compare_self := by grind
+
+instance: Std.LawfulEqOrd Unit where
+  eq_of_compare := by grind
+
+instance: Std.OrientedOrd Unit where
+  eq_swap := by grind [Ordering.swap]
+
+instance: Std.TransOrd Unit where
+  isLE_trans := by grind
+
+-- Constructors
+
+abbrev Vk.ctor: BytesCtor where
+  data := Unit
+  nBytes := 1
+  dataOrd := inferInstance
+  dataReflOrd := inferInstance
+  dataLawfulEqOrd := inferInstance
+  dataOrientedOrd := inferInstance
+  dataTransOrd := inferInstance
+
+class abbrev Vk.HasCtor [BytesCtors] := Bytes.HasCtor Vk.ctor
+
+abbrev Vk.id [BytesCtors] [Vk.HasCtor]: CtorId := Bytes.HasCtor.id Vk.ctor
+
+abbrev Vk.View [BytesCtors] [Vk.HasCtor] := BytesView Vk.id
+
+abbrev Sign.ctor: BytesCtor where
+  data := Unit
+  nBytes := 3
+  dataOrd := inferInstance
+  dataReflOrd := inferInstance
+  dataLawfulEqOrd := inferInstance
+  dataOrientedOrd := inferInstance
+  dataTransOrd := inferInstance
+
+class abbrev Sign.HasCtor [BytesCtors] := Bytes.HasCtor Sign.ctor
+
+abbrev Sign.id [BytesCtors] [Sign.HasCtor]: CtorId := Bytes.HasCtor.id Sign.ctor
+
+abbrev Sign.View [BytesCtors] [Sign.HasCtor] := BytesView Sign.id
+
+instance [BytesCtors] [Vk.HasCtor] [Sign.HasCtor]: CanSign Bytes where
+  vk sk :=
+    ({
+      data := (),
+      dataBytes := V[sk]
+    } : Vk.View).pack
+
+  sign sk nonce msg :=
+    ({
+      data := (),
+      dataBytes := V[sk, nonce, msg]
+    } : Sign.View).pack
+
+  verify vk msg sig :=
+    match sig.view? Sign.id with
+    | some { data := (), dataBytes := V[sk, _nonce, msg'] } =>
+      msg = msg' &&
+      vk = ({ data := (), dataBytes := V[sk] } : Vk.View).pack
+    | none => false
+
+theorem verify_sign
+  [BytesCtors] [Vk.HasCtor] [Sign.HasCtor]
+  (sk nonce msg: Bytes)
+  :
+    verify (vk sk) msg (sign sk nonce msg)
+  := by
+    simp only [verify, vk, sign]
+    grind
+
+def Sign.ctors := [Vk.ctor, Sign.ctor]
+
+instance [BytesCtors] [tc: Bytes.HasCtors Sign.ctors]: Bytes.HasCtor Vk.ctor := tc.tc (Fin.mk 0 (by simp [Sign.ctors]))
+instance [BytesCtors] [tc: Bytes.HasCtors Sign.ctors]: Bytes.HasCtor Sign.ctor := tc.tc (Fin.mk 1 (by simp [Sign.ctors]))
+
+-- Equational theory
+
+def Sign.attKnowsVk [BytesCtors] [Bytes.HasCtors Sign.ctors]: AttackerKnowledge where
+  pred p out :=
+    ∃ sk,
+      out = vk sk ∧
+      p sk
+  pred_scott_continuous := by
+    sorry
+
+def Sign.attKnowsSign [BytesCtors] [Bytes.HasCtors Sign.ctors]: AttackerKnowledge where
+  pred p out :=
+    ∃ sk nonce msg,
+      out = sign sk nonce msg ∧
+      p sk ∧
+      p nonce ∧
+      p msg
+  pred_scott_continuous := by
+    sorry
+
+def Sign.equationalTheory: EquationalTheory where
+  ctors := Sign.ctors
+  attackerKnowledge := [Sign.attKnowsVk, Sign.attKnowsSign]
+
+instance: EquationalTheory.CtorsEq Sign.equationalTheory Sign.ctors where pf := rfl
+
+instance: NeZero Sign.equationalTheory.ctors.length where
+  out := by simp [Sign.equationalTheory, Sign.ctors]
+
+theorem Sign.attacker_knows_vk
+  [EquationalTheories]
+  [HasEquationalTheory Sign.equationalTheory]
+  (sk: Bytes) (tr: Trace α)
+  :
+    sk.AttackerKnows tr →
+    (vk sk).AttackerKnows tr
+  := by
+    intro h_inp
+    apply Bytes.AttackerKnows.prove Sign.equationalTheory Sign.attKnowsVk
+    · simp [Sign.equationalTheory]
+    simp only [Sign.attKnowsVk]
+    grind
+
+theorem Sign.attacker_knows_sign
+  [EquationalTheories]
+  [HasEquationalTheory Sign.equationalTheory]
+  (sk nonce msg: Bytes) (tr: Trace α)
+  :
+    sk.AttackerKnows tr →
+    nonce.AttackerKnows tr →
+    msg.AttackerKnows tr →
+    (sign sk nonce msg).AttackerKnows tr
+  := by
+    intro h_inp h_nonce h_msg
+    apply Bytes.AttackerKnows.prove Sign.equationalTheory Sign.attKnowsSign
+    · simp [Sign.equationalTheory]
+    simp only [Sign.attKnowsSign]
+    grind
+
+-- Invariants
+
+def Vk.invariants [BytesCtors]: BytesCtorInvariants.Internal Vk.ctor where
+  well_formed := {
+    func := fun () V[sk] rec tr =>
+      rec sk tr
+    func_wf := by
+      intro data dataBytes rec1 rec2
+      let V[sk] := dataBytes
+      simp_all +arith
+  }
+
+  usage := {
+    func data dataBytes rec tr := Usage.nothing
+    func_wf := by grind
+  }
+  usage_later data dataBytes rec_wf rec_usg := by grind [GetUsageLaterT]
+
+  label := {
+    func := fun () V[sk] rec tr =>
+      Label.pub
+    func_wf := by
+      intro data dataBytes rec1 rec2
+      let V[sk] := dataBytes
+      simp_all +arith
+  }
+  label_later data dataBytes rec_wf rec_usg := by
+    let V[sk] := dataBytes
+    simp_all +arith [GetLabelLaterT]
+
+  invariant := {
+    func := fun () V[sk] rec tr =>
+      rec sk tr
+    func_wf := by
+      intro data dataBytes rec1 rec2
+      let V[sk] := dataBytes
+      simp_all +arith
+  }
+  invariant_implies_wellformed data dataBytes rec_inv rec_wf := by
+    let V[sk] := dataBytes
+    simp_all +arith [BytesInvariantImpliesBytesWellFormedT]
+  invariant_later data dataBytes rec := by
+    let V[sk] := dataBytes
+    simp_all +arith [BytesInvariantLaterT]
+    grind
+
+class abbrev Vk.HasInvariants [BytesCtors] [Vk.HasCtor] [BytesCtorsInvariants] := HasBytesInvariants (Vk.id) Vk.invariants
+
+class SignPred [BytesCtors] where
+  pred: [GetUsage] → [GetLabel] → Usage → Bytes → Bytes → ProofTrace → Prop
+  pred_later:
+    [BytesWellFormed] → [GetUsage] → [GetLabel] →
+    ∀ skUsg vk msg tr1 tr2,
+      vk.wellFormed tr1 →
+      msg.wellFormed tr1 →
+      tr1 ≤ tr2 →
+      pred skUsg vk msg tr1 →
+      pred skUsg vk msg tr2
+
+def Sign.invariants [BytesCtors] [SignPred] [Bytes.HasCtors Sign.ctors]: BytesCtorInvariants.Internal Sign.ctor where
+  well_formed := {
+    func := fun () V[sk, nonce, msg] rec tr =>
+      rec sk tr ∧
+      rec nonce tr ∧
+      rec msg tr
+    func_wf := by
+      intro data dataBytes rec1 rec2
+      let V[sk, nonce, msg] := dataBytes
+      simp_all +arith
+  }
+
+  usage := {
+    func data dataBytes rec tr := Usage.nothing
+    func_wf := by grind
+  }
+  usage_later data dataBytes rec_wf rec_usg := by grind [GetUsageLaterT]
+
+  label := {
+    func := fun () V[sk, nonce, msg] rec tr =>
+      Label.pub
+    func_wf := by
+      intro data dataBytes rec1 rec2
+      let V[sk, nonce, msg] := dataBytes
+      simp_all +arith
+  }
+  label_later data dataBytes rec_wf rec_usg := by
+    let V[sk, nonce, msg] := dataBytes
+    simp_all +arith [GetLabelLaterT]
+
+  invariant := {
+    func := fun () V[sk, nonce, msg] rec tr =>
+      rec sk tr ∧
+      rec nonce tr ∧
+      rec msg tr ∧
+      (
+        (
+          exists sk_usg,
+          -- Honest case:
+          -- - the key has the usage of signature key
+          -- TODO has usage
+          sk.usage tr = sk_usg ∧
+          sk_usg.type = "SigKey" ∧
+          -- - the custom (protocol-specific) invariant hold (authentication)
+          SignPred.pred sk_usg (vk sk) msg tr ∧
+          -- - the nonce is more secret than the signature key
+          --   (this is because the standard EUF-CMA security assumption on signatures
+          --   do not have any guarantees when the nonce is leaked to the attacker,
+          --   in practice knowing the nonce used to sign a message
+          --   can be used to obtain the private key,
+          --   hence this restriction)
+          (sk.label tr).canFlow (nonce.label tr) tr ∧
+          -- - the nonce has the correct usage (for the same reason as above)
+          -- nonce `has_usage tr` SigNonce
+          True
+        ) \/ (
+          -- Attacker case:
+          -- the attacker knows the signature key.
+          -- The message is not required to be known by the attacker:
+          -- the EUF-CMA security assumption on signatures doesn't guarantee
+          -- that in case of signature forgeries.
+          (sk.label tr).canFlow Label.pub tr
+        )
+      )
+
+    func_wf := by
+      intro data dataBytes rec1 rec2
+      let V[sk, nonce, msg] := dataBytes
+      simp_all +arith
+  }
+  invariant_implies_wellformed data dataBytes rec_inv rec_wf := by
+    let V[sk, nonce, msg] := dataBytes
+    simp_all +arith [BytesInvariantImpliesBytesWellFormedT]
+  invariant_later data dataBytes rec := by
+    let V[sk, nonce, msg] := dataBytes
+    simp_all +arith [BytesInvariantLaterT]
+    intro _ _ tr1 tr2
+    have := SignPred.pred_later (sk.usage tr1) (vk sk) msg tr1 tr2
+    grind
+
+class abbrev Sign.HasInvariants [BytesCtors] [Sign.HasCtor] [BytesCtorsInvariants] := HasBytesInvariants (Sign.id) Sign.invariants
+
+@[simp]
+theorem hash.wellFormed
+  [BytesCtors] [BytesCtorsInvariants]
+  [Sign.HasCtor] [Sign.HasInvariants]
+  (inp: Bytes) (tr: ProofTrace)
+  :
+    (hash inp).wellFormed tr = inp.wellFormed tr
+  := by
+    simp [hash, Bytes.wellFormed.eq, Sign.invariants]
+
+@[simp]
+theorem hash.label
+  [BytesCtors] [BytesCtorsInvariants]
+  [Sign.HasCtor] [Sign.HasInvariants]
+  (inp: Bytes) (tr: ProofTrace)
+  : (hash inp).label tr = inp.label tr
+  := by
+    simp [hash, Bytes.label.eq, Sign.invariants]
+
+@[simp]
+theorem hash.invariant
+  [BytesCtors] [BytesCtorsInvariants]
+  [Sign.HasCtor] [Sign.HasInvariants]
+  (inp: Bytes) (tr: ProofTrace)
+  :
+    (hash inp).invariant tr =
+    inp.invariant tr
+  := by
+    simp [hash, Bytes.invariant.eq, Sign.invariants]
+
+def Sign.EquationalTheoryInvariant [EquationalTheories]: EquationalTheoryInvariants Sign.equationalTheory where
+  invariant
+    | 0 => Sign.invariants
+
+instance
+  [EquationalTheories] [EquationalTheories.Invariants]
+  [HasEquationalTheory Sign.equationalTheory] [Sign.EquationalTheoryInvariant.Has]
+  : HasBytesInvariants Sign.id Sign.invariants :=
+  Sign.EquationalTheoryInvariant.mkHasBytesInvariants (Fin.mk 0 (by simp [Sign.equationalTheory, Sign.ctors]))
+
+-- Preserve publishability
+
+def Sign.attKnowsSign.preserves_publishability
+  [BytesCtors] [BytesCtorsInvariants]
+  [Bytes.HasCtors Sign.ctors] [Sign.HasInvariants]: Sign.attKnowsSign.PreservesPublishability :=
+  by
+    simp only [AttackerKnowledge.PreservesPublishability, Sign.attKnowsSign]
+    intro out tr ⟨inp, ⟨ h_out, h_inp ⟩⟩
+    subst h_out
+    simp_all [Bytes.Publishable]
+
+def Sign.PreservesPublishability
+  [EquationalTheories] [EquationalTheories.Invariants]
+  [HasEquationalTheory Sign.equationalTheory]
+  [Sign.EquationalTheoryInvariant.Has]
+  : EquationalTheory.PreservesPublishability Sign.equationalTheory where
+  pf := by
+    unfold Sign.equationalTheory
+    simp
+    exact attKnowsSign.preserves_publishability
+
+end DY
