DY/Kleene.lean
@@ -1,0 +1,217 @@
+/-
+  This module formalizes Kleene's fixpoint theorem
+  https://en.wikipedia.org/wiki/Kleene_fixed-point_theorem
+-/
+
+namespace DY.Kleene
+
+def Set (α: Type u) := α → Prop
+
+instance: HasSubset (Set α) where
+  Subset set1 set2 :=
+    ∀ x, set1 x → set2 x
+
+@[ext]
+theorem Set.ext
+  {α: Type u}
+  (set1 set2: Set α)
+  :
+  (∀ x, set1 x ↔ set2 x) →
+  set1 = set2
+  := by
+    intro h
+    funext
+    simp_all
+
+def Chain (α: Type u) := Nat → Set α
+
+def Chain.IsDirected {α: Type u} (chain: Chain α): Prop :=
+  ∀ i j, i ≤ j → (chain i) ⊆ (chain j)
+
+def Chain.union (chain: Chain α): Set α :=
+  fun x => ∃ n, chain n x
+
+def Chain.map (f: Set α → Set α) (chain: Chain α): Chain α :=
+  fun n => fun x => f (chain n) x
+
+def IsScottContinuous {α: Type u} (f: Set α → Set α): Prop :=
+  ∀ chain: Chain α,
+    chain.IsDirected →
+    f (chain.union) = (chain.map f).union
+
+def IsMonotonic {α: Type u} (f: Set α → Set α): Prop :=
+  ∀ set1 set2: Set α,
+    set1 ⊆ set2 →
+    f set1 ⊆ f set2
+
+theorem isScottContinuous_implies_isMonotonic
+  {α: Type u} (f: Set α → Set α):
+  IsScottContinuous f →
+  IsMonotonic f
+  := by
+    intro h_scott set1 set2 h_subset x
+    let chain: Chain α := fun n => if n = 0 then set1 else set2
+    have h_chain_directed: chain.IsDirected := by
+      subst chain
+      intros i j
+      by_cases i = 0 <;>
+      by_cases j = 0 <;>
+      simp_all [Subset]
+    have h_chain_scott := h_scott chain h_chain_directed
+    have h_chain_scott_left: chain.union = set2 := by
+      ext x
+      simp only [Chain.union]
+      constructor
+      · intro ⟨ n, h_n ⟩
+        by_cases n = 0
+        · apply h_subset x
+          grind
+        · grind
+      · intro h
+        exists 1
+    have h_chain_scott_right: (chain.map f).union = (fun x => f set1 x ∨ f set2 x) := by
+      ext x
+      subst chain
+      simp_all only [Chain.union, Chain.map, iff_or_self]
+      intro
+      exists 0
+    rewrite [h_chain_scott_left] at h_chain_scott
+    rewrite [h_chain_scott_right] at h_chain_scott
+    rewrite [h_chain_scott]
+    grind
+
+def mkWeakestFixpointAux {α: Type u} (f: Set α → Set α): Chain α :=
+  fun n =>
+    if n = 0 then
+      fun _ => False
+    else
+      f (mkWeakestFixpointAux f (n-1))
+
+def mkWeakestFixpoint {α: Type u} (f: Set α → Set α): Set α :=
+  (mkWeakestFixpointAux f).union
+
+theorem mkWeakestFixpointAux_monotonic_consecutive
+  {α: Type u}
+  (f: Set α → Set α)
+  (h_scott: IsScottContinuous f)
+  (i: Nat)
+  : mkWeakestFixpointAux f i ⊆ mkWeakestFixpointAux f (i+1)
+  := by
+    induction i with
+    | zero => simp [mkWeakestFixpointAux, Subset]
+    | succ i ih =>
+      unfold mkWeakestFixpointAux
+      exact isScottContinuous_implies_isMonotonic f h_scott (mkWeakestFixpointAux f i) (mkWeakestFixpointAux f (i+1)) ih
+
+theorem mkWeakestFixpointAux_monotonic
+  {α: Type u}
+  (f: Set α → Set α)
+  (h_scott: IsScottContinuous f)
+  (i j: Nat)
+  :
+  i ≤ j →
+  mkWeakestFixpointAux f i ⊆ mkWeakestFixpointAux f j
+  := by
+    intro h_ij
+    induction h_ij with
+    | refl => simp [Subset]
+    | step =>
+      rename_i j' _ _
+      have := mkWeakestFixpointAux_monotonic_consecutive f h_scott j'
+      simp_all [Subset]
+
+theorem mkWeakestFixpoint_is_fixpoint
+  {α: Type u}
+  (f: Set α → Set α)
+  (h_scott: IsScottContinuous f)
+  : f (mkWeakestFixpoint f) = mkWeakestFixpoint f
+  := by
+    unfold mkWeakestFixpoint
+    have := h_scott (mkWeakestFixpointAux f) (mkWeakestFixpointAux_monotonic f h_scott)
+    rewrite [this]
+    ext x
+    simp [Chain.union, Chain.map]
+    have: ∀ n, f (mkWeakestFixpointAux f n) x = mkWeakestFixpointAux f (n+1) x := by
+      intro n
+      conv =>
+        rhs
+        unfold mkWeakestFixpointAux
+        simp
+    simp only [this]
+    constructor
+    · rintro ⟨ n, h_n ⟩
+      exists n+1
+    · rintro ⟨ n, h_n ⟩
+      by_cases n = 0
+      · unfold mkWeakestFixpointAux at h_n
+        subst_vars
+        simp at h_n
+      · exists n-1
+        unfold mkWeakestFixpointAux
+        unfold mkWeakestFixpointAux at h_n
+        simp_all
+
+theorem mkWeakestFixpoint_is_weakest_aux
+  {α: Type u}
+  (f: Set α → Set α)
+  (h_scott: IsScottContinuous f)
+  (set: Set α)
+  (n: Nat)
+  :
+  (f set) ⊆ set →
+  mkWeakestFixpointAux f n ⊆ set
+  := by
+    induction n with
+    | zero =>
+      unfold mkWeakestFixpointAux
+      simp [Subset]
+    | succ n ih =>
+      unfold mkWeakestFixpointAux
+      have := isScottContinuous_implies_isMonotonic f h_scott (mkWeakestFixpointAux f n) set
+      simp
+      intro h
+      simp_all [Subset]
+
+theorem mkWeakestFixpoint_is_weakest
+  {α: Type u}
+  (f: Set α → Set α)
+  (h_scott: IsScottContinuous f)
+  (set: Set α)
+  :
+  (f set) ⊆ set →
+  mkWeakestFixpoint f ⊆ set
+  := by
+    intro h
+    simp [mkWeakestFixpoint, Chain.union, Subset]
+    intro x n
+    have := mkWeakestFixpoint_is_weakest_aux f h_scott set n h
+    simp_all [Subset]
+
+def combine {α: Type u} (fs: List (Set α → Set α)) (set: Set α): Set α :=
+  fun x =>
+    ∃ f,
+      f ∈ fs ∧
+      f set x
+
+theorem combine_isScottContinuous
+  {α: Type u}
+  (fs: List (Set α → Set α))
+  (h_fs: ∀ f, f ∈ fs → IsScottContinuous f)
+  : IsScottContinuous (combine fs)
+  := by
+    intro chain h_chain
+    unfold combine
+    ext x
+    constructor
+    · intro ⟨f, ⟨h_f1, h_f2⟩⟩
+      have := h_fs f h_f1 chain h_chain
+      simp_all [Chain.union, Chain.map]
+      grind
+    · intro h
+      have ⟨n, f, ⟨h_f1, h_f2⟩⟩ := h
+      have := h_fs f h_f1 chain h_chain
+      exists f
+      simp_all only [Chain.union, Chain.map, true_and]
+      exists n
+
+end DY.Kleene
